[Checkpoint] Oracle refinement equality problem.
The problem I encountered is oracle_ok says there exists a place to split the oracle but there is no way to relate this to an oracle that is used in an execution.

I will go back to consuming a part of a oracle to amend this problem.

src/HoareL1.v
@@ -7,8 +7,8 @@ Set Implicit Arguments.
 
 (** ** Hoare logic *)
 Definition precond := oracle -> @pred addr addr_dec (set value).
-Definition postcond {T: Type} := T -> @pred addr addr_dec (set value).
-Definition crashcond := @pred addr addr_dec (set value).
+Definition postcond {T: Type} := oracle -> disk (set value) -> T -> @pred addr addr_dec (set value).
+Definition crashcond := oracle -> disk (set value) -> @pred addr addr_dec (set value).
 
 
 Definition hoare_triple {T: Type} (pre: precond) (p: prog T) (post: @postcond T) (crash: crashcond):=
@@ -18,21 +18,21 @@ Definition hoare_triple {T: Type} (pre: precond) (p: prog T) (post: @postcond T)
         exec o d p ret /\
         ((exists d' r,
              ret = Finished d' r
-             /\ post r d') \/
+             /\ post o d r d') \/
          (exists d',
-             ret = Crashed d' /\ crash d')))%type.
+             ret = Crashed d' /\ crash o d d')))%type.
 
 
   
 Notation
-  "<< o >> pre p << r >> post crash" :=
+  "<< o >> pre p << d , r >> post crash" :=
   (forall F, hoare_triple
           (fun o d => (F * pre * [[ oracle_ok p o d ]]) d)%pred
           p%pred
-          (fun r => F * post)%pred
-          (F * crash)%pred)
-    (at level 10, o at next level, pre at next level, p at next level, r at next level, post at next level, crash at next level,
-     format "'[v' '[  ' '<<' o '>>' '//' '[' pre ']' '//' '[' p ']' ']' '//' '[  ' '<<' r '>>' '//' '[' post ']' '//' '[' crash ']' ']' ']'").
+          (fun o d r => F * post)%pred
+          (fun o d => F * crash)%pred)
+    (at level 10, o at next level, d at next level, pre at next level, p at next level, r at next level, post at next level, crash at next level,
+     format "'[v' '[  ' '<<' o '>>' '//' '[' pre ']' '//' '[' p ']' ']' '//' '[  ' '<<' d ',' r '>>' '//' '[' post ']' '//' '[' crash ']' ']' ']'").
 
 (*
 Notation
@@ -63,8 +63,8 @@ Theorem hoare_triple_weaken_post_weak:
   hoare_triple pre p post crash ->
   (forall  o d r,
       pre o d ->
-      post r =p=>
-      post' r) ->
+      post o d r =p=>
+      post' o d r) ->
   hoare_triple pre p post' crash.
 Proof.
   unfold hoare_triple; intros;
@@ -80,9 +80,9 @@ Qed.
 Theorem hoare_triple_weaken_post_strong:
   forall T (p: prog T) pre (post post': postcond) crash,
   hoare_triple pre p post crash ->
-  (forall (r: T),
-      post r =p=>
-      post' r) ->
+  (forall o d (r: T),
+      post o d r =p=>
+      post' o d r) ->
   hoare_triple pre p post' crash.
 Proof.
   intros; eapply hoare_triple_weaken_post_weak; eauto.
@@ -93,8 +93,8 @@ Theorem hoare_triple_weaken_crash_weak:
   hoare_triple pre p post crash ->
   (forall o d,
       pre o d ->
-      crash =p=>
-      crash') ->
+      crash o d =p=>
+      crash' o d) ->
   hoare_triple pre p post crash'.
 Proof.
   unfold  hoare_triple; intros;
@@ -110,7 +110,7 @@ Qed.
 Theorem hoare_triple_weaken_crash_strong:
   forall T (p: prog T) pre post (crash crash': crashcond),
   hoare_triple pre p post crash ->
-  crash =p=> crash' ->
+  (forall o d, crash o d =p=> crash' o d) ->
   hoare_triple pre p post crash'.
 Proof.
   intros; eapply hoare_triple_weaken_crash_weak; eauto.
@@ -270,6 +270,7 @@ Proof.
   apply in_app_iff; eauto.
 Qed.
 
+
 Theorem hoare_triple_pimpl :
     forall T1 T2 (p1: prog T1) (p2: T1 -> prog T2) (pre: precond) pre1 post1 pre2 post2 crash1 crash2,
       hoare_triple pre1 p1 post1 crash1 ->
@@ -281,21 +282,31 @@ Theorem hoare_triple_pimpl :
             pre1 o1 d) ->
       (forall o1 d,
          pre1 o1 d ->
-         (forall o2 r, post1 r =p=> pre2 o2)) ->
+         (forall o2 r, post1 o1 d r =p=> pre2 o2)) ->
       (forall o1 d r,
          pre1 o1 d ->
-         (forall o2, post1 r =p=> pre2 o2) ->
+         (forall o2, post1 o1 d r =p=> pre2 o2) ->
           hoare_triple pre2 (p2 r) post2 crash2) ->
     (forall o d,
       pre1 o d ->
-      crash1 =p=> crash2) ->
+      crash1 o d =p=> crash2 o d) ->
+    (forall o1 o2 d1 d2 r1 r2,
+        pre1 o1 d1 ->
+        post1 o1 d1 r1 d2 ->
+        pre2 o2 d2 ->
+        post2 o2 d2 r2  =p=> post2 (o1++o2) d1 r2) ->
+    (forall o1 o2 d1 d2 r1,
+        pre1 o1 d1 ->
+        post1 o1 d1 r1 d2 ->
+        pre2 o2 d2 ->
+        crash2 o2 d2  =p=> crash2 (o1++o2) d1) ->
     hoare_triple pre (Bind p1 p2) post2 crash2.
 Proof.
   unfold hoare_triple; intros.
   edestruct H0; eauto; cleanup.
   edestruct H; eauto; cleanup.
-  specialize H1 with (1:=H7).
-  specialize H3 with (1:=H7).
+  specialize H1 with (1:=H9).
+  specialize H3 with (1:=H9).
   split_ors.
   - (* p1 Finished *)    
     edestruct H2; eauto.
@@ -303,14 +314,24 @@ Proof.
     cleanup.
     split_ors; cleanup.
     + (* p2 Finished *)
-      eexists. intuition eauto.
+      clear H8.
+      eexists; split; eauto.
+      left; do 2 eexists; intuition eauto.
+      eapply H4; eauto.
+      eapply H1; eauto.
     + (* p2 Crashed *)
+      clear H8.
       eexists. intuition eauto.
+      right; eexists; intuition eauto.
+      eapply H5; eauto.
+      eapply H1; eauto.
   - (* p1 Crashed *)
+    split_ors; cleanup.
     eexists. intuition eauto.
     cleanup; rewrite app_nil_r;
       econstructor; eauto.
-    apply exec_crash_in in H5; intuition.   
+    cleanup; rewrite app_nil_r; eauto.
+    apply exec_crash_in in H7; intuition.   
 Qed.
 
 
@@ -452,79 +473,101 @@ Proof.
 Qed.
 
 Theorem bind_ok:
-  forall T T' (p1: prog T) (p2: T -> prog T') pre1 post1 crash1 pre2 post2 crash2,
+  forall T T' (p1: prog T) (p2: T -> prog T') pre1 post1 crash1 pre2 post2 crash2 crash3,
   << o >>
-   pre1
+   (pre1 o)
    p1
-  << r >>
-   (post1 r)
-   crash1 ->
-  (forall F d r,
-      (F * pre1)%pred d ->
-      post1 r =p=> pre2) ->
+  << d, r >>
+   (post1 o d r)
+   (crash1 o d) ->
+  (forall o o',
+      pre1 (o++o') =p=> pre1 o ) ->
+  (forall F o o' d r,
+      (F * pre1 o)%pred d ->
+      post1 o d r =p=> pre2 o') ->
   (forall F o d d' r,
-      (F * pre1)%pred d ->
-      exec o d p1 (Finished d' r) ->
-      (F * post1 r)%pred d' ->
+      (F * pre1 o)%pred d ->
+      (F * post1 o d r)%pred d' ->
       << o >>
-         pre2
+         (pre2 o)
          (p2 r)
-       << r >>
-       (post2 r)
-       crash2) ->
+       << d, r >>
+       (post2 o d r)
+       (crash2 o d)) ->
+  (forall F d1 d2 r1 r2 o1 o2,
+      (F * pre1 o1)%pred d1 ->
+      (F * post1 o1 d1 r1)%pred d2 ->
+      (F * pre2 o2)%pred d2 ->
+      post2 o2 d2 r2 =p=> post2 (o1++o2) d1 r2) ->
+  (forall F o d,
+      (F * pre1 o)%pred d ->
+      crash1 o d =p=> crash3 o d) ->
+  (forall F d1 d2 r1 o1 o2,
+      (F * pre1 o1)%pred d1 ->
+      (F * post1 o1 d1 r1)%pred d2 ->
+      (F * pre2 o2)%pred d2 ->
+      crash2 o2 d2 =p=> crash3 (o1++o2) d1) ->
   << o >>
-     pre1
+     (pre1 o)
      (Bind p1 p2)
-  << r >>
-     (post2 r)
-     (crash1 \/ crash2).
+  << d, r >>
+     (post2 o d r)
+     (crash3 o d).
 Proof.
   unfold hoare_triple; intros.
   simpl in *; destruct_lifts; cleanup.
+  rewrite H0 in H6.
   edestruct H; eauto.
-  pred_apply' H2; norm.
-  cancel.
-  eauto.
+  pred_apply' H6; cancel; eauto.
+  apply sep_star_comm.
+  
   cleanup.
   split_ors; cleanup.
-  - specialize H5 with (1:=H3).
-    edestruct H1; eauto.
-    pred_apply' H9; norm.
+  - specialize H9 with (1:=H7).
+    edestruct H2; eauto.
+    pred_apply' H13; norm.
     cancel.
-    rewrite H0;
+    rewrite H1;
       intuition eauto.
-    cancel.
+    cancel; eauto.
     intuition eauto.
+
     cleanup.
     split_ors; cleanup;
-      eexists; split; intuition eauto.
+    eexists; split; intuition eauto.
+    left; do 2 eexists; intuition eauto.
+    pred_apply; cancel.
+    eapply H3; eauto.
+    erewrite <- H1; eauto.
+    
     right; eexists; intuition eauto.
     pred_apply; cancel.
-    apply pimpl_or_r; intuition eauto.
-  - specialize H6 with (1:=H3); cleanup.
+    eapply H5; eauto.
+    erewrite <- H1; eauto.
+  - specialize H10 with (1:=H7); cleanup.
     rewrite app_nil_r.
     eexists; split; intuition eauto.
     right; eexists; intuition eauto.
     pred_apply; cancel.
-    apply pimpl_or_r; intuition eauto.
+    eauto.
 Qed.
 
 
 Theorem crash_weaken:
   forall T (p: prog T) pre post crash1 crash2,
   << o >>
-   pre
+   (pre o)
    p
-  << r >>
+  << d, r >>
    (post r)
-   crash1 ->
-  (crash1 =p=> crash2) ->
+   (crash1 o d) ->
+  (forall o d, crash1 o d =p=> crash2 o d) ->
   << o >>
-     pre
+     (pre o)
      p
-  << r >>
+  << d, r >>
      (post r)
-     crash2.
+     (crash2 o d).
 Proof.
   unfold hoare_triple; intros.
   edestruct H; eauto.
@@ -539,18 +582,18 @@ Qed.
 Theorem post_weaken:
   forall T (p: prog T) pre post1 post2 crash,
   << o >>
-   pre
+   (pre o)
    p
-  << r >>
+  << d, r >>
    (post1 r)
-   crash ->
+   (crash o d)  ->
   (forall r, post1 r =p=> post2 r) ->
   << o >>
-     pre
+     (pre o)
      p
-  << r >>
+  << d, r >>
      (post2 r)
-     crash.
+     (crash o d).
 Proof.
   unfold hoare_triple; intros.
   edestruct H; eauto.
@@ -564,18 +607,18 @@ Qed.
 Theorem pre_strengthen:
   forall T (p: prog T) pre1 pre2 post crash,
   << o >>
-   pre1
+   (pre1 o)
    p
-  << r >>
+  << d, r >>
    (post r)
-   crash ->
-  (pre2 =p=> pre1) ->
+   (crash o d) ->
+  (forall o, pre2 o =p=> pre1 o) ->
   << o >>
-     pre2
+     (pre2 o)
      p
-  << r >>
+  << d, r >>
      (post r)
-     crash.
+     (crash o d).
 Proof.
   unfold hoare_triple; intros.
   edestruct H; eauto.
@@ -585,21 +628,22 @@ Qed.
 Theorem add_frame:
   forall T (p: prog T) pre post crash F,
   << o >>
-   pre
+   (pre o)
    p
-  << r >>
+  << d, r >>
    (post r)
-   crash ->
+   (crash o d) ->
   << o >>
-     (F * pre)
+     (F * pre o)
      p
-  << r >>
+  << d, r >>
      (F * post r)
-     (F * crash).
+     (F * crash o d).
 Proof.
   unfold hoare_triple; intros.
   edestruct H; eauto.
   pred_apply' H0; cancel; eauto.
+  rewrite sep_star_assoc; cancel.
   cleanup; split_ors; cleanup;
     eexists; intuition eauto.
   left; do 2 eexists; intuition eauto.
@@ -611,17 +655,17 @@ Qed.
 Theorem extract_exists:
   forall T V (p: prog T) pre post crash,
   (forall (v:V), << o >>
-   (pre v)
+   (pre o v)
    p
-  << r >>
+  << d, r >>
    (post r)
-   crash) ->
+   (crash o d)) ->
   << o >>
-     (exists v, pre v)
+     (exists v, pre o v)
      p
-  << r >>
+  << d, r >>
      (post r)
-     crash.
+     (crash o d).
 Proof.
   unfold hoare_triple; intros.
   destruct_lifts.
