src/Layer1to2Refinement.v
@@ -1,119 +1,109 @@
 Require Import Primitives Layer1 BlockAllocator.
-Require Import Layer2 SimulationLayer.
+Require Import Layer2 SimulationLayer Layer1to2RefinementDefinitions.
 Require Import FunctionalExtensionality Omega.
 
 Section Layer1to2Refinement.
-  
-  Fixpoint compile {T} (p2: Layer2.prog T) : Layer1.prog T :=
-    match p2 with
-    | Read a => read a
-    | Write a v => write a v
-    | Alloc v => alloc v
-    | Free a => free a
-    | Ret v => Layer1.Ret v
-    | Bind px py => Layer1.Bind (compile px) (fun x => compile (py x))
-    end.
 
-  
-  Fixpoint oracle_refines_to T (d1: Layer1.state) (p: Layer2.prog T)  (o1: Layer1.oracle) (o2: Layer2.oracle) : Prop :=
-    match p with
-    | Alloc v =>
-      if (in_dec Layer1.token_dec Layer1.Crash o1) then
-        o2 = {| token_list := [Crash]; refinement_length := length o1 |}
-      else
-        let sv := Disk.read d1 0 in
-        match sv with
-        | Some v =>
-          let bits := bits (value_to_bits v) in
-          let index := get_first_zero bits in
-          
-          if lt_dec index block_size then
-            o2 = {| token_list := [BlockNum index]; refinement_length := length o1 |}
-          else
-            o2 = {| token_list := [DiskFull]; refinement_length := length o1 |}
-        | None => False
-        end
-    | @Bind T1 T2 p1 p2 =>
-
-      exists d1',
-      (Layer1.exec o1 d1 (compile p1) (Crashed d1') /\
-         oracle_refines_to T1 d1 p1 o1 o2) \/
-      (exists r o1' o1'' o2' o2'' ret,
-         o1 = o1'++o1'' /\
-         Layer1.exec o1' d1 (compile p1) (Finished d1' r) /\
-         Layer1.exec o1'' d1' (compile (p2 r)) ret /\
-         oracle_refines_to T1 d1 p1 o1' o2' /\
-         oracle_refines_to T2 d1' (p2 r) o1'' o2'' /\
-         o2 = {| token_list:= token_list o2'++ token_list o2'';
-                 refinement_length := refinement_length o2' + refinement_length o2'' |})
-    | _ =>
-      if (in_dec Layer1.token_dec Layer1.Crash o1) then
-        o2 = {| token_list := [Crash]; refinement_length := length o1 |}
-      else
-        o2 = {| token_list := [Cont]; refinement_length := length o1 |}
-    end.
-
-  Definition refines_to d1 d2 :=
-    exists F, (F * rep d2)%pred d1.
-
-  Definition compilation_of T p1 p2 :=
-    p1 = @compile T p2.
-
-  Definition low := Build_LTS (list Layer1.token) Layer1.state Layer1.prog Layer1.exec.
-
-  Definition high := Build_LTS Layer2.oracle Layer2.state Layer2.prog Layer2.exec.
-
-  Lemma star_split:
-    forall (AT : Type) (AEQ : EqDec AT) (V : Type)
-      (p q : @pred AT AEQ V) (m : @mem AT AEQ V),
-      (p * q)%pred m ->
-      exists m1 m2, mem_disjoint m1 m2 /\ p m1 /\ q m2 /\ mem_union m1 m2 = m.
+  Lemma length_lt_prefix:
+    forall T (l1 l2 l3 l4: list T),
+      l1++l2=l3++l4 ->
+      length l1 < length l3 ->
+      exists l1', l3 = l1++l1' /\ l1' <> [].
   Proof.
-    intros; unfold sep_star in *; rewrite sep_star_is in *;
-      destruct H; cleanup; eauto.
-    do 2 eexists; intuition eauto.
+    induction l1; simpl in *; intros; eauto.
+    destruct l3; simpl in *.
+    inversion H0.
+    eexists; split; eauto.
+    congruence.
+    destruct l3; simpl in *.
+    inversion H0.
+    inversion H; subst.
+    edestruct IHl1; eauto.
+    omega.
+    destruct H1; subst.
+    eexists; eauto.
   Qed.
-  
-  Lemma rep_eq:
-    forall d s1 s2 F F',
-      (F * rep s1)%pred d ->
-      (F' * rep s2)%pred d ->
-      s1 = s2.
-  Proof.
-    intros.
-    extensionality k.
-    unfold rep in *; simpl in *.
-    
-    destruct_lift H; destruct_lift H0.
-    eapply_fresh ptsto_valid' in H.
-    eapply_fresh ptsto_valid in H5; cleanup.
-    eapply mem_union_addr in Hx; eauto.
-    eapply mem_union_addr in Hx0; eauto.
-    all: try solve [apply mem_disjoint_comm; eauto].
-    rewrite mem_union_comm in Hx, Hx0; eauto.
-    all: try solve [apply mem_disjoint_comm; eauto].
-    unfold set in *; simpl in *.
-    rewrite H3 in Hx; cleanup.
-                             
-    destruct_fresh (nth k (bits (value_to_bits dummy)) 0).
-    rewrite H9, H11; eauto.
-    
-    destruct (value_to_bits dummy); simpl in *.
-    unfold valid_bitlist in *; cleanup.
-    destruct (nth_in_or_default k bits 0); [|cleanup; omega].
-    apply H7 in i; cleanup.
-    destruct n; cleanup; try omega.
-    specialize (H8 _ D).
-    specialize (H10 _ D); cleanup; eauto.
-    eapply mem_union_addr in H8; eauto.
-    eapply mem_union_addr in H10; eauto.
-    all: try solve [apply mem_disjoint_comm; eauto].
-    rewrite mem_union_comm in H8, H10; eauto.
-    all: try solve [apply mem_disjoint_comm; eauto].
-    unfold set in *; simpl in *.
-    rewrite H3 in H8; cleanup; eauto.    
-  Qed.      
 
+  Lemma oracle_ok_app_exec_nil:
+    forall T (p: Layer1.prog T) o1 o2 s ret,
+      Layer1.exec o1 s p ret ->
+      oracle_ok p (o1++o2) s ->
+      o2=[].
+  Proof.
+     induction p; simpl; intros;
+       try solve [  unfold oracle_ok in *; intuition; apply app_eq_unit in H1;
+                    split_ors; cleanup; eauto; invert_exec ].
+     invert_exec;
+     unfold oracle_ok in H1; cleanup;
+    fold (@oracle_ok T) in *;
+    fold (@oracle_ok T') in *.
+    cleanup.
+      Search app nil.
+    split_ors; cleanup.
+    
+  Lemma oracle_ok_bind_split:
+    forall T T' (p1: Layer1.prog T) (p2: T -> Layer1.prog T') o1 o2 sl sl' r ret,
+      Layer1.exec o1 sl p1 (Finished sl' r) ->
+      Layer1.exec o2 sl' (p2 r) ret ->
+      oracle_ok (Layer1.Bind p1 p2) (o1 ++ o2) sl ->
+      oracle_ok p1 o1 sl /\
+      oracle_ok (p2 r) o2 sl'.      
+  Proof.
+    simpl; intros.
+    unfold oracle_ok in H1; cleanup;
+    fold (@oracle_ok T) in *;
+    fold (@oracle_ok T') in *.
+    destruct (lt_dec (length o1) (length x)).
+    -
+      eapply length_lt_prefix in H1; eauto; cleanup.
+      
+      Search app length lt.
+    specialize IHp with (1:= H0)(2:=H3).
+    repeat rewrite app_length; cleanup.
+Admitted.
+
+  Axiom oracle_ok_exec_app_nil:
+    forall T (p: Layer1.prog T) o1 o2 s ret,
+      Layer1.exec (o1++o2) s p ret ->
+      oracle_ok p o1 s ->
+      o2=[].
+
+  (* XXX: We need oracle lengths to extract oracle equalities *) 
+  Axiom layer1_exec_finished_then_oracle_length_eq :
+    forall T (p: Layer1.prog T) s o1 o2 s'1 s'2 r1 r2,
+      Layer1.exec o1 s p (Finished s'1 r1) ->
+      Layer1.exec o2 s p (Finished s'2 r2) ->
+      o1 = o2.
+
+  Axiom layer1_finished_not_crashed_app:
+    forall T (p1: Layer1.prog T) o1 o2 s s' s'' r,
+       Layer1.exec o1 s p1 (Finished s' r) ->
+       ~ Layer1.exec (o1++o2) s p1 (Crashed s'').
+
+  Axiom layer1_exec_preserves_refines_to:
+    forall T (p2: Layer2.prog T) o1 s1 s1',
+      Layer1.exec o1 s1 (compile p2) s1' ->
+      (exists s2, refines_to s1 s2) ->
+      (exists s2', refines_to (extract_state s1') s2').
+  
+
+  Axiom oracle_refines_to_deterministic:
+    forall T (p: Layer2.prog T) s o o1 o2,
+      oracle_refines_to T s p o o1 ->
+      oracle_refines_to T s p o o2 ->
+      o1 = o2.
+
+  Lemma oracle_ok_nonempty:
+    forall T (p: Layer1.prog T) s,
+      ~oracle_ok p [] s.
+  Proof.
+    unfold not, oracle_ok;
+    induction p; simpl; intros; try intuition congruence.
+    cleanup.
+    symmetry in H0; apply app_eq_nil in H0; cleanup; eauto.
+  Qed.
+  Hint Resolve oracle_ok_nonempty.
+  
   (*
   Lemma oracle_refinement_deterministic:
     forall T p2 ol1 ol2 oh sl1 sl2 p1 sl1' sl2', (* sh1 sh2 sh1' sh2' ,
@@ -222,100 +212,147 @@ Section Layer1to2Refinement.
         eassign
    *)
 
-  Axiom finished_crash_not_in :
-    forall T o s (p: Layer1.prog T) s' r,
-      Layer1.exec o s p (Finished s' r) ->
-      ~ In Layer1.Crash o.
-
-  Axiom crashed_crash_in :
-    forall T o s (p: Layer1.prog T) s',
-      Layer1.exec o s p (Crashed s') ->
-      In Layer1.Crash o.
-
-  Axiom layer1_exec_deterministic :
-    forall T o s (p: Layer1.prog T) s' s'',
-      Layer1.exec o s p s' ->
-      Layer1.exec o s p s'' ->
-      s' = s''.
-
-  Lemma exec_low_to_high_oracle:
+  Arguments oracle_ok T p o s : simpl never.
+  Arguments oracle_refines_to T d1 p o1 o2 : simpl never.
+  
+  Lemma Axiom1:
     forall T p2 p1 ol sl sl',
+      (exists sh, refines_to sl sh) ->
+      oracle_ok p1 ol sl ->
       Layer1.exec ol sl p1 sl' ->
       (forall d, sl' <> Failed d) ->
       compilation_of T p1 p2 ->
       exists oh, oracle_refines_to T sl p2 ol oh.
   Proof.
-    unfold compilation_of;
-      induction p2; simpl; intros; cleanup;
-      try solve [ exists (match sl' with
-         | Crashed _ => {| token_list:= [Crash]; refinement_length := length ol |}
-         | Finished _ _ => {| token_list:= [Cont]; refinement_length := length ol |}
-         | Failed _ => {| token_list:= []; refinement_length := length ol |}
-         end); intros;
-        destruct sl'; simpl in *; [
-      eapply finished_crash_not_in in H;
-        destruct (in_dec token_dec Layer1.Crash ol); intuition tauto |
-      eapply crashed_crash_in in H;
-      destruct (in_dec token_dec Layer1.Crash ol); intuition tauto |
-      exfalso; eapply H0; eauto] ].
+    unfold refines_to, compilation_of;
+    induction p2; simpl; intros; cleanup.
 
+    - (* Read *)
+      edestruct read_ok.
+      pred_apply' H; cancel; eauto.
+      cleanup; split_ors;
+      cleanup; destruct_lifts; eauto.
+    - (* Write *)
+      edestruct write_ok.
+      pred_apply' H; cancel; eauto.
+      cleanup; split_ors;
+        cleanup; destruct_lifts; eauto.
+      split_ors; cleanup; eauto.
+        
     - (* Alloc *)
-      exists (match sl' with
-         | Crashed _ => {| token_list:= [Crash]; refinement_length := length ol |}
-         | Finished _ r =>
-           match r with
-           | Some a => {| token_list:= [BlockNum a]; refinement_length := length ol |}
-           | None => {| token_list:= [DiskFull]; refinement_length := length ol |}
-           end
-         | Failed _ => {| token_list:= []; refinement_length := length ol |}
-         end); intros.
-      destruct sl'; simpl in *.
-      eapply finished_crash_not_in in H;
-        destruct (in_dec token_dec Layer1.Crash ol); try intuition tauto.
-      (* XXX: We need to know about the behavior of alloc here *)
-      admit.
-      eapply crashed_crash_in in H;
-        destruct (in_dec token_dec Layer1.Crash ol); intuition tauto.
-      exfalso; eapply H0; eauto.
-      
+      edestruct alloc_ok.
+      pred_apply' H; cancel; eauto.
+      cleanup; split_ors;
+        cleanup; destruct_lifts; 
+          split_ors; cleanup; eauto.
+    - (* Free *)
+      edestruct free_ok.
+      pred_apply' H; cancel; eauto.
+      cleanup; split_ors;
+        cleanup; destruct_lifts; eauto;
+          split_ors; cleanup; eauto.
+    - (* Ret *)
+      destruct sl';
+      unfold oracle_refines_to; simpl;
+        destruct (in_dec token_dec Crash ol); eauto.
     - (* Bind *)
       invert_exec; cleanup.      
       + (* Finished *)
+        unfold oracle_ok in H1; cleanup.
+        fold (@oracle_ok T) in H5.
+        fold (@oracle_ok T') in H6.
+
+        eapply_fresh oracle_ok_finished_length in H2; eauto.
+        eapply ListUtils.app_split_length_eq_l in Hx; eauto; cleanup.
         edestruct IHp2; eauto.
         intros d Hx; inversion Hx.
-        edestruct H; eauto.
-        exists ({| token_list:= token_list x3 ++ token_list x4; refinement_length := refinement_length x3 + refinement_length x4 |}), x1.
-        right; intros.
-        do 6 eexists; intuition eauto.
+        edestruct layer1_exec_preserves_refines_to; try apply H2; eauto.
+        unfold refines_to; eauto.
+        edestruct H; eauto; simpl in *.
+        exists (x1++x7).
+        unfold oracle_refines_to; simpl; fold oracle_refines_to.
+        split.
+        unfold oracle_ok; simpl;
+        fold (@oracle_ok T); fold (@oracle_ok T').
+
+        do 2 eexists; intuition eauto.
+        do 2 eexists; intuition eauto.
+        
+        exfalso; eapply layer1_finished_not_crashed_app in H2; eauto.
+        exfalso; eapply layer1_finished_not_crashed_app in H2; eauto.
+        eapply exec_finished_deterministic in H2; eauto; cleanup.
+        do 2 eexists; intuition eauto.
+        
       + (* Crashed *)
+        unfold oracle_ok in H1; cleanup.
+        fold (@oracle_ok T) in H4.
+        fold (@oracle_ok T') in H5.
+
         split_ors; cleanup.
-        * edestruct IHp2; eauto.
+        * eapply_fresh oracle_ok_exec_app_nil in H1; eauto; cleanup.
+          rewrite app_nil_r in *.
+          edestruct IHp2; eauto.
           intros d Hx; inversion Hx.
-        * edestruct IHp2; eauto.
+          exists x2.
+          unfold oracle_refines_to; simpl; fold oracle_refines_to.
+          split.
+          unfold oracle_ok; simpl;
+          fold (@oracle_ok T); fold (@oracle_ok T').
+
+          do 2 eexists; intuition eauto.
+          rewrite app_nil_r; eauto.
+          do 2 eexists; intuition eauto.
+          rewrite app_nil_r; eauto.
+          specialize H5 with (1:= H8).
+          
+          exfalso; eapply oracle_ok_nonempty; eauto.
+        
+        * eapply_fresh oracle_ok_finished_length in H4; eauto.
+          eapply ListUtils.app_split_length_eq_l in Hx; eauto; cleanup.
+          edestruct IHp2; eauto.
           intros d Hx; inversion Hx.
-          edestruct H; eauto.
-          do 2 eexists; right; intros.
-          do 6 eexists; intuition eauto.
+          edestruct layer1_exec_preserves_refines_to; try apply H1; eauto.
+          unfold refines_to; eauto.
+          edestruct H; eauto; simpl in *.
+          exists (x3++x7).
+          unfold oracle_refines_to; simpl; fold oracle_refines_to.
+          split.
+          unfold oracle_ok; simpl;
+          fold (@oracle_ok T); fold (@oracle_ok T').
+
+          do 2 eexists; intuition eauto.
+          do 2 eexists; intuition eauto.
+
+          exfalso; eapply layer1_finished_not_crashed_app in H1; eauto.
+          exfalso; eapply layer1_finished_not_crashed_app in H1; eauto.
+          eapply exec_finished_deterministic in H1; eauto; cleanup.
+          do 2 eexists; intuition eauto.
+        
       + (* Failed *)
-        exfalso; eapply H1; eauto.
-  Abort.
+        exfalso; eapply H3; eauto.
+  Qed.
 
 (*
-  Lemma exec_high_to_low_oracle:
+  Lemma Axiom2:
     forall T p2 oh sl sh sh',
       refines_to sl sh ->
+      (exists o, oracle_ok (compile p2) o sl) ->
       Layer2.exec oh sh p2 sh' ->
       exists ol, oracle_refines_to T sl p2 ol oh.
   Proof.
     induction p2; simpl; intros.
     - (* Read *)
-      inversion H0; cleanup.
-      eexists; intros.
+      inversion H1; clear H1; cleanup.
       
       + (* Finished *)
         unfold refines_to in *; cleanup.
-        eapply read_ok in H; cleanup.
-        split_ors; destruct_lifts; cleanup.
+        edestruct read_ok.
+        pred_apply' H; norm.
+        cancel.
+        intuition eauto.
+
+        cleanup.
+        split_ors; destruct_lifts; cleanup; eauto.
         edestruct H4.
         
         split_ors; cleanup.
@@ -326,299 +363,510 @@ Section Layer1to2Refinement.
 Abort.
 *)
 
-  (* XXX: We need oracle lengths to extract oracle equalities *) 
-  Axiom layer1_exec_finished_then_oracle_length_eq :
-    forall T (p: Layer1.prog T) s o1 o2 s'1 s'2 r1 r2,
-      Layer1.exec o1 s p (Finished s'1 r1) ->
-      Layer1.exec o2 s p (Finished s'2 r2) ->
-      length o1 = length o2.
-
-  Lemma app_split_length_eq :
-    forall T (l1 l2 l1' l2': list T),
-      l1++l2 = l1'++l2' ->
-      length l1 = length l1' ->
-      l1 = l1' /\ l2 = l2'.
+  Theorem sbs_read :
+    forall a,
+      StrongBisimulationForProgram
+        layer1_lts layer2_lts
+        compilation_of
+        refines_to
+        oracle_refines_to
+        (Read a).              
   Proof.
-    induction l1; simpl; intros.
-    symmetry in H0.
-    apply length_zero_iff_nil in H0; cleanup.
-    simpl; eauto.
-
-    destruct l1'; simpl in *.
-    inversion H0.
-    cleanup.
-    edestruct IHl1; eauto; cleanup; eauto.
-  Qed.
+    constructor; intros.
     
-  Theorem sbs :
-    forall valid_h,
-      StrongBisimulation
-        low high
-        (refines_to_valid refines_to valid_h)
-        (compiles_to_valid (fun _ _ => True) compilation_of)
-        valid_h
-        (fun _ _ => True)
-        compilation_of refines_to
-        oracle_refines_to.              
-  Proof.
-    constructor.
-    intros T p1 p2.
-    generalize dependent p1.
-    induction p2; intros.
-    { (* Read *)
-      unfold refines_to_valid, refines_to,
-      compiles_to_valid, compilation_of, oracle_refines_to in *; intros.
-      simpl in *;
+    unfold refines_to,
+    compiles_to_valid, compilation_of in *; intros.
+    simpl in *;
       split.
-      + (* Low to High *)
-        intros; cleanup.
-        * (* Crashed *)
-          rewrite H4 in *.
-          eapply_fresh (read_ok a) in H3; cleanup.
-          eapply_fresh layer1_exec_deterministic in H6; eauto; cleanup.        
-          split_ors; cleanup.
-          --
-            destruct_lifts.
-            tauto.
-          --
-            destruct_lifts.
-            eexists; split.
-            eapply ExecOpCrash; eauto.
-            intros T p1 p2 Hx; inversion Hx.
-            simpl in *.
-            repeat split; eauto.
-            intuition (cleanup; eauto).
-            eapply_fresh rep_eq in H0; eauto; cleanup; eauto.
-        * (* Finished *)
-          rewrite H4 in *.
-          eapply_fresh (read_ok a) in H3; cleanup.
-          eapply_fresh layer1_exec_deterministic in H6; eauto; cleanup.        
-          split_ors; cleanup.
-          --
-            destruct_lifts.
-            eexists; split.
-            econstructor; eauto.
-            simpl in *.
-            repeat split; eauto.
-            
-            intuition (cleanup; eauto).
-            apply star_split in H0; cleanup.
-            unfold rep in *.
-            destruct_lift H7.          
-            erewrite H11; eauto; simpl.
-            apply nth_overflow; simpl.
-            destruct (value_to_bits dummy); simpl.
-            unfold valid_bitlist in *; cleanup; eauto.
-            
-            intros; cleanup.
-            eapply_fresh rep_eq in H0; eauto; cleanup; eauto.
-          --
-            destruct_lifts.
-            exfalso; eauto.
-
-      + (*High to low*)
-        intros; cleanup.
-        * (* Crashed *)
-        eapply (read_ok a) in H3; cleanup.
-        split_ors; cleanup.
-        --
-          destruct_lifts.
-          exfalso; eauto.
-        --
-          destruct_lifts.
-          inversion H6; sigT_eq; simpl in *; cleanup.
+    
+    + (* Low to High *)
+      intros; cleanup.
+      edestruct (read_ok a); eauto.
+      pred_apply' H. norm.
+      cancel.
+      unfold oracle_refines_to in *; cleanup;
+      intuition eauto.
+      cleanup.
+      eapply_fresh deterministic_prog in H2; eauto; cleanup.        
+      split_ors; cleanup;
+      destruct_lifts;
+      match goal with
+      |[H: oracle_refines_to _ _ _ ?o _,
+        H0: oracle_refines_to _ _ _ ?o _ |- _] =>
+       eapply oracle_refines_to_deterministic in H; eauto; cleanup
+      end.
+      
+      * (* Finished *)
+        eexists; split.
+        econstructor; eauto.
+        simpl in *.
+        repeat split; eauto.
+          
+        intuition (cleanup; eauto).
+        unfold rep in *.
+        destruct_lifts.          
+        symmetry; eauto.
+  
+      * (* Crashed *)
+        eexists; split.
+        econstructor; eauto.
+        simpl in *.
+        repeat split; eauto.
+          
+    + (*High to low*)
+      intros; cleanup.
+      edestruct (read_ok a); cleanup.
+      pred_apply' H; norm.
+      cancel.
+      unfold oracle_refines_to in *.
+      intuition eauto.
+        
+      split_ors; cleanup;
+      destruct_lifts;
+      match goal with
+      |[H: oracle_refines_to _ _ _ ?o _,
+        H0: oracle_refines_to _ _ _ ?o _ |- _] =>
+       eapply oracle_refines_to_deterministic in H; eauto; cleanup
+      end;
+      match goal with
+      | [H: Layer2.exec _ _ _ _ |- _] =>
+        inversion H; sigT_eq; simpl in *; cleanup
+      end.
+      * (* Finished *)
+        eexists; split.
+        eauto.
+        simpl in *.
+        repeat split; eauto.
+        
+        intuition (cleanup; eauto).
+        unfold rep in *.
+        destruct_lifts;          
+        symmetry; eauto.
+          
+      * (* Crashed *)
           eexists; split.
           eauto.
           simpl in *.
           repeat split; eauto.
-          intuition (cleanup; eauto).
-          eapply_fresh rep_eq in H2; eauto;
-            cleanup; eauto.
-          
-        * (* Finished *)
-          eapply (read_ok a) in H3; cleanup.
-          split_ors; cleanup.
-          --
-            destruct_lifts.
-            inversion H6; sigT_eq; simpl in *; cleanup.
-            eexists; split.
-            eauto.
-            simpl in *.
-            repeat split; eauto.
+  Qed.
 
-            intuition (cleanup; eauto).
-            apply star_split in H2; cleanup.
-            unfold rep in *.
-            destruct_lift H7.          
-            erewrite H11; eauto; simpl.
-            apply nth_overflow; simpl.
-            destruct (value_to_bits dummy); simpl.
-            unfold valid_bitlist in *; cleanup; eauto.
-          
-            intros; cleanup.
-            eapply_fresh rep_eq in H2; eauto;
-              cleanup; eauto.
-          --
-            destruct_lifts.
-            exfalso; eauto.
-    }
-    { (* Write *) 
-      admit.
-    }
-    { (* Alloc *)
-      admit.
-    }
-    { (* Free *)
-      admit.
-    }
-    { (* Ret *)
-      admit.
-    }
-    { (* Bind *)
-      unfold compilation_of in *; simpl in *; cleanup.
-      split; intros.
-      - (* Low to High *)
-        invert_exec.
-        + (* Finished *)
-          split_ors; cleanup.
-          * (* XXX: If Finished with o, then cannot crash with o++o' *)
-            admit.
-          *            
-            eapply_fresh layer1_exec_finished_then_oracle_length_eq in H8; eauto.
-            apply app_split_length_eq in H6; eauto; cleanup.
-            eapply_fresh layer1_exec_deterministic in H8; eauto; cleanup.
-            eapply_fresh layer1_exec_deterministic in H9; eauto; cleanup.
-          
-            edestruct IHp2; eauto.
-            unfold compiles_to_valid;
-            eexists; split; eauto.
-            edestruct H5; eauto; simpl in *; cleanup; try tauto.
-            clear H5 H6.
-            simpl in *.
-            destruct H14; eauto; cleanup.
-            
-            edestruct H; try reflexivity; eauto.
-            unfold compiles_to_valid;
-            eexists; split; eauto.
-            edestruct H5; eauto; simpl in *; cleanup; try tauto.
-            clear H5 H6.
-            simpl in *.
-            destruct H18; eauto; cleanup.
-            
-            eexists; split.
-            econstructor; eauto.
-            
-            simpl in *.
-            intuition eauto.
-        + (* Crashed *)
-          destruct H5; cleanup.
-          * (* First Crashed *)
-            split_ors; cleanup.
-            --
-              edestruct IHp2; eauto.
-              unfold compiles_to_valid;
-              eexists; split; eauto.
-              edestruct H8; eauto; simpl in *; cleanup; try tauto.
-              clear H8 H9.
-              simpl in *.
-              
-              eexists; split.
-              eapply ExecBindCrash; eauto.
-              simpl in *; intuition eauto.
-            -- (* XXX: If Finished with o, then cannot crash with o++o' *)
-              admit.
-          * (* Second Crashed *)
-             split_ors; cleanup.
-             -- (* XXX: If Finished with o, then cannot crash with o++o' *)
-              admit.
-             --
-               eapply_fresh layer1_exec_finished_then_oracle_length_eq in H8; eauto.
-               apply app_split_length_eq in H6; eauto; cleanup.
-               eapply_fresh layer1_exec_deterministic in H8; eauto; cleanup.
-               eapply_fresh layer1_exec_deterministic in H9; eauto; cleanup.
-               
-               edestruct IHp2; eauto.
-               unfold compiles_to_valid;
-               eexists; split; eauto.
-               edestruct H5; eauto; simpl in *; cleanup; try tauto.
-               clear H5 H6.
-               simpl in *.
-               destruct H14; eauto; cleanup.
-            
-               edestruct H; try reflexivity; eauto.
-               unfold compiles_to_valid;
-               eexists; split; eauto.
-               edestruct H5; eauto; simpl in *; cleanup; try tauto.
-               clear H5 H6.
-               simpl in *.
-               
-               eexists; split.
-               econstructor; eauto.
-               
-               simpl in *.
-               intuition eauto.
-        + (* Failed *)
-          destruct H5; cleanup.
-          * (* First Failed *)
-            split_ors; cleanup.
-            --
-              eapply layer1_exec_deterministic in H6;
-              eauto; inversion H6.
-            -- (* XXX: If Finished with o, then cannot crash with o++o' *)
-              admit.
-          * (* Second Failed *)
-            split_ors; cleanup.
-            -- (* XXX: If Finished with o, then cannot crash with o++o' *)
-              admit.
-            --
-              eapply_fresh layer1_exec_finished_then_oracle_length_eq in H8; eauto.
-              apply app_split_length_eq in H6; eauto; cleanup.
-              eapply_fresh layer1_exec_deterministic in H8; eauto; cleanup.
-              eapply_fresh layer1_exec_deterministic in H9; eauto; cleanup.
+  Theorem sbs_write :
+    forall a v,
+      StrongBisimulationForProgram
+        layer1_lts layer2_lts
+        compilation_of refines_to
+        oracle_refines_to
+        (Write a v).              
+  Proof.
+    constructor; intros.
+    cleanup; try tauto.    
+    unfold refines_to, compiles_to_valid, compilation_of in *; intros.
+    simpl in *; split.
 
-            edestruct IHp2; eauto.
-            unfold compiles_to_valid;
-            eexists; split; eauto.
-            edestruct H5; eauto; simpl in *; cleanup; try tauto.
-            clear H5 H6.
-            simpl in *.
-            destruct H14; eauto; cleanup.
-            
-            edestruct H; try reflexivity; eauto.
-            unfold compiles_to_valid;
-            eexists; split; eauto.
-            edestruct H5; eauto; simpl in *; cleanup; try tauto.
-            clear H5 H6.
-            simpl in *.
-            
-            eexists; split.
-            econstructor; eauto.
-            
-            simpl in *.
-            intuition eauto.
-            
-      - (* High to Low *)
-        unfold compiles_to_valid in H1; cleanup.
-        inversion H5; sigT_eq; clear H5.
-        + (* Finished *)
-          split_ors; cleanup.
-          (* XXX: HERE *)
+    + (* Low to High *)
+      intros; cleanup.
+      edestruct write_ok; eauto.
+      pred_apply' H. norm.
+      cancel.
+      unfold oracle_refines_to in *.
+      intuition eauto.
+      cleanup.
+      eapply_fresh deterministic_prog in H2; eauto; cleanup.        
+      split_ors; cleanup;
+      destruct_lifts;
+      try split_ors; cleanup;
+      match goal with
+      |[H: oracle_refines_to _ _ _ ?o _,
+        H0: oracle_refines_to _ _ _ ?o _ |- _] =>
+       eapply oracle_refines_to_deterministic in H; eauto; cleanup
+      end.
+        
+      * (* Finished 1 *)
+        eexists; split.
+        eapply ExecWriteFail; eauto.
+        simpl in *.
+        repeat split; eauto.
+
+      * (* Finished 2 *)
+        eexists; split.
+        econstructor; eauto.
+        simpl in *.
+        repeat split; eauto.
+          
+      * (* Crashed 1 *)
+        eexists; split.
+        econstructor; eauto.
+        simpl in *.
+        repeat split; eauto.
+
+      * (* Crashed 2 *)
+        eexists; split.
+        econstructor; eauto.
+        simpl in *.
+        repeat split; eauto.
+          
+    + (*High to low*)
+      intros; cleanup.
+      edestruct write_ok; eauto.
+      pred_apply' H. norm.
+      cancel.
+      unfold oracle_refines_to in *.
+      intuition eauto.
+      cleanup.
+      
+      split_ors; cleanup;
+      destruct_lifts;
+      split_ors; cleanup;
+      match goal with
+      |[H: oracle_refines_to _ _ _ ?o _,
+        H0: oracle_refines_to _ _ _ ?o _ |- _] =>
+       eapply oracle_refines_to_deterministic in H; eauto; cleanup
+      end;
+      match goal with
+      | [H: Layer2.exec _ _ _ _ |- _] =>
+        inversion H; sigT_eq; simpl in *; cleanup
+      end;
+      try congruence.
+
+      * (* Finished 1 *)
+        eexists; split.
+        eauto.
+        simpl in *.
+        repeat split; eauto.
+
+      * (* Finished 2 *)
+        eexists; split.
+        eauto.
+        simpl in *.
+        repeat split; eauto.
+        
+      * (* Crashed 1 *)
+        eexists; split.
+        eauto.
+        simpl in *.
+        repeat split; eauto.
+
+      * (* Crashed 2 *)
+        eexists; split.
+        eauto.
+        simpl in *.
+        repeat split; eauto.
+Qed.
+
+  Theorem sbs_free :
+    forall a,
+    StrongBisimulationForProgram
+      layer1_lts layer2_lts
+      compilation_of refines_to
+      oracle_refines_to
+      (Free a).              
+  Proof.
+    constructor; intros.
+    cleanup; try tauto.    
+    unfold refines_to, compiles_to_valid, compilation_of in *; intros.
+    simpl in *; split.
+
+    + (* Low to High *)
+      intros; cleanup.
+      edestruct free_ok; eauto.
+      pred_apply' H. norm.
+      cancel.
+      unfold oracle_refines_to in *.
+      intuition eauto.
+      cleanup.
+      eapply_fresh deterministic_prog in H2; eauto; cleanup.        
+      split_ors; cleanup;
+      destruct_lifts;
+      try split_ors; cleanup;
+      match goal with
+      |[H: oracle_refines_to _ _ _ ?o _,
+        H0: oracle_refines_to _ _ _ ?o _ |- _] =>
+       eapply oracle_refines_to_deterministic in H; eauto; cleanup
+      end.
+        
+      * (* Finished  *)
+        eexists; split.
+        econstructor; eauto.
+        simpl in *.
+        repeat split; eauto.
+          
+      * (* Crashed 1 *)
+        eexists; split.
+        econstructor; eauto.
+        simpl in *.
+        repeat split; eauto.
+        
+      * (* Crashed 2 *)
+        eexists; split.
+        econstructor; eauto.
+        simpl in *.
+        repeat split; eauto.
+          
+    + (*High to low*)
+      intros; cleanup.
+      edestruct free_ok; eauto.
+      pred_apply' H. norm.
+      cancel.
+      unfold oracle_refines_to in *.
+      intuition eauto.
+      cleanup.
+      
+      split_ors; cleanup;
+      destruct_lifts;
+      try split_ors; cleanup;
+      match goal with
+      |[H: oracle_refines_to _ _ _ ?o _,
+        H0: oracle_refines_to _ _ _ ?o _ |- _] =>
+       eapply oracle_refines_to_deterministic in H; eauto; cleanup
+      end;
+      match goal with
+      | [H: Layer2.exec _ _ _ _ |- _] =>
+        inversion H; sigT_eq; simpl in *; cleanup
+      end;
+      try congruence.
+
+      * (* Finished *)
+        eexists; split.
+        eauto.
+        simpl in *.
+        repeat split; eauto.
+        
+      * (* Crashed 1 *)
+        eexists; split.
+        eauto.
+        simpl in *.
+        repeat split; eauto.
+
+      * (* Crashed 2 *)
+        eexists; split.
+        eauto.
+        simpl in *.
+        repeat split; eauto.
+  Qed.
+ 
+
+  Theorem sbs_ret :
+    forall T (v: T),
+    StrongBisimulationForProgram
+      layer1_lts layer2_lts
+      compilation_of refines_to
+      oracle_refines_to
+      (Ret v).              
+  Proof.
+        constructor; intros.
+    cleanup; try tauto.    
+    unfold refines_to, compiles_to_valid, compilation_of in *; intros.
+    simpl in *; split.
+
+    + (* Low to High *)
+      intros; cleanup.
+      invert_exec; cleanup;
+      unfold oracle_refines_to in *;
+      cleanup; simpl in *;
+      try split_ors; intuition; try congruence.
+
+      * (* Finished  *)
+        eexists; split.
+        econstructor; eauto.
+        simpl in *.
+        repeat split; eauto.
+          
+      * (* Crashed *)
+        eexists; split.
+        econstructor; eauto.
+        simpl in *.
+        repeat split; eauto.
+        
+          
+    + (*High to low*)
+      intros; cleanup.
+      
+      match goal with
+      | [H: Layer2.exec _ _ _ _ |- _] =>
+        inversion H; sigT_eq; simpl in *; cleanup
+      end;
+      try congruence;
+      unfold oracle_refines_to, oracle_ok in *;
+      cleanup; simpl in *;
+      repeat (split_ors; cleanup; simpl in *);
+      intuition; try congruence.
+
+      * (* Finished *)
+        eexists; split.
+        eauto.
+        simpl in *.
+        repeat split; eauto.
+        
+      * (* Crashed *)
+        eexists; split.
+        econstructor; eauto.
+        intros; congruence.
+        simpl in *.
+        repeat split; eauto.
+  Qed.
+
+   Theorem sbs_alloc :
+     forall v,
+      StrongBisimulationForProgram
+        layer1_lts layer2_lts
+        compilation_of refines_to
+        oracle_refines_to
+        (Alloc v).              
+  Proof.
+    constructor; intros.
+    cleanup; try tauto.    
+    unfold refines_to, compiles_to_valid, compilation_of in *; intros.
+    simpl in *; split.
+
+    + (* Low to High *)
+      intros; cleanup.
+      edestruct alloc_ok; eauto.
+      pred_apply' H. norm.
+      cancel.
+      unfold oracle_refines_to in *.
+      intuition eauto.
+      cleanup.
+      eapply_fresh deterministic_prog in H2; eauto; cleanup.        
+      split_ors; cleanup;
+      destruct_lifts;
+      try split_ors; cleanup;
+      match goal with
+      |[H: oracle_refines_to _ _ _ ?o _,
+        H0: oracle_refines_to _ _ _ ?o _ |- _] =>
+       eapply oracle_refines_to_deterministic in H; eauto; cleanup
+      end.
+        
+      * (* Finished  *)
+        eexists; split.
+        econstructor; eauto.
+        simpl in *.
+        repeat split; eauto.
+        
+      * (* Finished  *)
+        eexists; split.
+        econstructor; eauto.
+        simpl in *.
+        repeat split; eauto.
+          
+      * (* Crashed 1 *)
+        eexists; split.
+        econstructor; eauto.
+        simpl in *.
+        repeat split; eauto.
+        
+      * (* Crashed 2 *)
+        eexists; split.
+        econstructor; eauto.
+        simpl in *.
+        repeat split; eauto.
+          
+    + (*High to low*)
+      intros; cleanup.
+      edestruct alloc_ok; eauto.
+      pred_apply' H. norm.
+      cancel.
+      unfold oracle_refines_to in *.
+      intuition eauto.
+      cleanup.
+      
+      split_ors; cleanup;
+      destruct_lifts;
+      try split_ors; cleanup;
+      match goal with
+      |[H: oracle_refines_to _ _ _ ?o _,
+        H0: oracle_refines_to _ _ _ ?o _ |- _] =>
+       eapply oracle_refines_to_deterministic in H; eauto; cleanup
+      end;
+      match goal with
+      | [H: Layer2.exec _ _ _ _ |- _] =>
+        inversion H; sigT_eq; simpl in *; cleanup
+      end;
+      try congruence.
+
+      * (* Finished *)
+        eexists; split.
+        eauto.
+        simpl in *.
+        repeat split; eauto.
+        
+      * (* Finished *)
+        eexists; split.
+        eauto.
+        simpl in *.
+        repeat split; eauto.
+        
+      * (* Crashed 1 *)
+        eexists; split.
+        eauto.
+        simpl in *.
+        repeat split; eauto.
+
+      * (* Crashed 2 *)
+        eexists; split.
+        eauto.
+        simpl in *.
+        repeat split; eauto.
+  Qed.
+
+  Theorem sbs_bind:
+    forall T1 T2 (p1: Layer2.prog T1) (p2: T1 -> Layer2.prog T2),
+      StrongBisimulationForProgram layer1_lts layer2_lts
+          compilation_of refines_to oracle_refines_to p1 ->
+    (forall t,
+      StrongBisimulationForProgram layer1_lts layer2_lts
+        compilation_of refines_to oracle_refines_to 
+        (p2 t)) ->
+    StrongBisimulationForProgram layer1_lts layer2_lts
+          compilation_of refines_to oracle_refines_to (Layer2.Bind p1 p2).
+  Proof.
+    intros.
+    edestruct H.
+    constructor; intros.
+    unfold compilation_of, oracle_refines_to in *;
+    simpl in *; cleanup;
+    fold oracle_refines_to in *.
+    unfold oracle_ok in *; simpl in *; cleanup.
+    fold (@oracle_ok T1) in *; fold (@oracle_ok T2) in *.
+
+    split; intros.
+    - (* Low to High *)
+      invert_exec; cleanup; intuition.
+      eapply_fresh oracle_ok_finished_length in H9; eauto.
+      eapply ListUtils.app_split_length_eq_l in Hx; eauto; cleanup.
+      specialize H4 with (1:= H9).
+      (* Oct 18: Fix oracle_refines_to definition for Bind *)
   Admitted.
+    
+  Hint Resolve sbs_alloc sbs_free sbs_read sbs_ret sbs_write sbs_bind.
+  
+  Theorem sbs :
+      StrongBisimulation
+        layer1_lts layer2_lts
+        compilation_of refines_to
+        oracle_refines_to.              
+  Proof.
+    apply bisimulation_restrict_prog.
+    induction p; eauto.
+  Qed.
+
+  Hint Resolve sbs.
 
   Theorem sbs_general:
-    forall valid_h valid_prog_h,
-      StrongBisimulation
-        low high
-        (refines_to_valid refines_to valid_h)
+    forall valid_state_h valid_prog_h,
+      exec_compiled_preserves_validity layer1_lts layer2_lts
+    compilation_of (refines_to_valid refines_to valid_state_h) ->
+    exec_preserves_validity layer2_lts valid_state_h ->
+      StrongBisimulationForValidStates
+        layer1_lts layer2_lts
+        (refines_to_valid refines_to valid_state_h)
         (compiles_to_valid valid_prog_h compilation_of)
-        valid_h
+        valid_state_h
         valid_prog_h
         compilation_of refines_to
         oracle_refines_to.  
   Proof.
     intros.
-    eapply bisimulation_weaken_valid_prog; [|apply sbs].
-    intuition.
+    eapply bisimulation_restrict_state; eauto.
   Qed.
     
 End Layer1to2Refinement.
