src/Layer2.v
@@ -1,5 +1,5 @@
-Require Import Primitives Disk Simulation.
-Require Import Layer1 BlockAllocator.
+Require Import Primitives Disk Simulation SimulationLayer.
+Require Import Layer1.
 Require Import Omega FunctionalExtensionality Memx.
 Import ListNotations.
 Close Scope pred_scope.
@@ -11,13 +11,11 @@ Section Layer2.
   | BlockNum : addr -> token
   | DiskFull : token
   | Cont : token
-  | Crash : token.
+  | Crash1 : token
+  | Crash2 : token
+  | CrashAlloc: addr -> token.
 
-  Record oracle :=
-    {
-      token_list : list token;
-      refinement_length : nat;
-    }.
+  Definition oracle := list token.
     
   Definition state := disk value.
   
@@ -32,56 +30,75 @@ Section Layer2.
   Inductive exec :
     forall T, oracle -> state -> prog T -> @Result state T -> Prop :=
   | ExecRead : 
-      forall o d a,
-        token_list o = [Cont] ->
-        exec o d (Read a) (Finished d (d a))
+      forall d a,
+        exec [Cont] d (Read a) (Finished d (d a))
              
   | ExecWriteSucc :
-      forall o d a v,
-        token_list o = [Cont] ->
+      forall d a v,
         d a <> None ->
-        exec o d (Write a v) (Finished (upd d a v) (Some tt))
+        exec [Cont] d (Write a v) (Finished (upd d a v) (Some tt))
 
   | ExecWriteFail :
-      forall o d a v,
-        token_list o = [Cont] ->
+      forall d a v,
         d a = None ->
-        exec o d (Write a v) (Finished d None)
+        exec [Cont] d (Write a v) (Finished d None)
 
   | ExecAllocSucc :
-      forall o d a v,
-        token_list o = [BlockNum a] ->
+      forall d a v,
         d a = None ->
-        exec o d (Alloc v) (Finished (upd d a v) (Some a))
+        exec [BlockNum a] d (Alloc v) (Finished (upd d a v) (Some a))
 
   | ExecAllocFail :
-      forall o d v,
-        token_list o = [DiskFull] ->
-        exec o d (Alloc v) (Finished d None)
+      forall d v,
+        exec [DiskFull] d (Alloc v) (Finished d None)
 
   | ExecFree :
-      forall o d a,
-        token_list o = [Cont] ->
-        exec o d (Free a) (Finished (delete d a) tt)
+      forall d a,
+        exec [Cont] d (Free a) (Finished (delete d a) tt)
              
   | ExecRet :
-      forall o d T (v: T),
-        token_list o = [Cont] ->
-        exec o d (Ret v) (Finished d v)
+      forall d T (v: T),
+        exec [Cont] d (Ret v) (Finished d v)
 
   | ExecBind :
       forall T T' (p1: prog T) (p2: T -> prog T')
         o1 o2 d d1 r ret,
         exec o1 d p1 (Finished d1 r) ->
         exec o2 d1 (p2 r) ret ->
-        exec {| token_list := token_list o1 ++ token_list o2;
-                refinement_length := refinement_length o1 + refinement_length o2; |} d (Bind p1 p2) ret
+        exec (o1 ++ o2) d (Bind p1 p2) ret
              
-  | ExecOpCrash :
-      forall T (p: prog T) o d,
-        token_list o = [Crash] ->
-        (forall T1 (p1: prog T1) p2, p <> Bind p1 p2) ->
-        exec o d p (Crashed d)
+  | ExecReadCrash :
+      forall d a,
+        exec [Crash1] d (Read a) (Crashed d)
+
+  | ExecWriteCrashBefore :
+      forall d a v,
+        exec [Crash1] d (Write a v) (Crashed d)
+
+  | ExecWriteCrashAfter :
+      forall d a v,
+        exec [Crash2] d (Write a v) (Crashed (upd d a v))
+
+  | ExecAllocCrashBefore :
+      forall d v,
+        exec [Crash1] d (Alloc v) (Crashed d)
+
+  | ExecAllocCrashAfter :
+      forall d a v,
+        d a = None ->
+        exec [CrashAlloc a] d (Alloc v) (Crashed (upd d a v))
+             
+  | ExecFreeCrashBefore :
+      forall d a,
+        exec [Crash1] d (Free a) (Crashed d)
+
+  | ExecFreeCrashAfter :
+      forall d a,
+        exec [Crash2] d (Free a) (Crashed (delete d a))
+             
+  | ExecRetCrash :
+      forall T d (a: T),
+        exec [Crash1] d (Ret a) (Crashed d)
              
   | ExecBindCrash :
       forall T T' (p1: prog T) (p2: T -> prog T')
@@ -95,7 +112,10 @@ Section Layer2.
         exec o d p1 (Failed d1) ->
         exec o d (Bind p1 p2) (Failed d1).
   (* TODO: add Failed cases *)
+
+  Definition layer2_lts := Build_LTS oracle state prog exec.
   
 End Layer2.
 
 Notation "x <- p1 ; p2" := (Bind p1 (fun x => p2))(right associativity, at level 60).
+Hint Constructors exec.
