src/SimulationLayer.v
@@ -68,29 +68,34 @@ Definition compiles_to_valid {Prog_L Prog_H: Type -> Type}
     compilation_of T pl ph /\
     valid_prog_h T ph.
 
-Definition oracle_refines_to_valid
-           {State1 State2 Oracle1 Oracle2: Type} {Op1 Op2: Type -> Type}
-           (oracle_refines_to: forall T, State1 -> Op2 T -> Oracle1 -> Oracle2 -> Prop)
-           (refines_to: State1 -> State2 -> Prop)
-           (compilation_of: forall T, Op1 T -> Op2 T -> Prop)
-           (valid_oracle2: forall T, Oracle2 -> State2 -> Op2 T -> Prop)
-           T (o1: Oracle1) (st1: State1) (p1: Op1 T) :=
-  forall st2 p2,
-    refines_to st1 st2 ->
-    compilation_of T p1 p2 ->
-    exists o2, oracle_refines_to T st1 p2 o1 o2 /\
-    valid_oracle2 T o2 st2 p2.
+Definition exec_preserves_validity lts valid_state :=
+    forall T (p: Prog lts T) o s ret,
+      valid_state s ->
+      exec lts T o s p ret ->
+      valid_state (extract_state ret).
 
+Definition exec_compiled_preserves_validity lts1 lts2 (compilation_of: forall T, Prog lts1 T -> Prog lts2 T -> Prop) valid_state :=
+    forall T (p1: Prog lts1 T) (p2: Prog lts2 T) o s ret,
+      compilation_of T p1 p2 ->
+      valid_state s ->
+      exec lts1 T o s p1 ret ->
+      valid_state (extract_state ret).
+
+(*
+  valid_state: This predicate restrict the statement to "well-formed" states.
+  valid_op: This predicate restrict programs to valid ones
+  R: This is the actual simulation relation
+*)
 Record SelfSimulation (lts: LTS)
        (valid_state: State lts -> Prop)
-       (valid_op: forall T, Prog lts T -> Prop)
+       (valid_prog: forall T, Prog lts T -> Prop)
        (R: State lts -> State lts -> Prop) :=
   {
     self_simulation_correct:
       forall T o p s1 s1' s2,
         valid_state s1 ->
         valid_state s2 ->
-        valid_op T p ->
+        valid_prog T p ->
         (exec lts) T o s1 p s1' ->
         R s1 s2 ->
         exists s2',
@@ -102,7 +107,7 @@ Record SelfSimulation (lts: LTS)
           valid_state (extract_state s2') ;
   }.
 
-Record StrongBisimulation
+Record StrongBisimulationForValidStates
        (lts1 lts2 : LTS)
        (valid_state1 : State lts1 -> Prop)
        (valid_prog1: forall T, Prog lts1 T -> Prop)
@@ -113,7 +118,7 @@ Record StrongBisimulation
        (oracle_refines_to: forall T, State lts1 -> Prog lts2 T -> Oracle lts1 -> Oracle lts2 -> Prop)
   :=
   {
-    strong_bisimulation_correct:
+    strong_bisimulation_for_valid_states_correct:
       (forall T p1 p2 s1 s2 o1 o2,
           valid_state1 s1 ->
           valid_prog1 T p1 ->
@@ -143,6 +148,153 @@ Record StrongBisimulation
                 valid_state1 (extract_state s1') /\ valid_state2 (extract_state s2')))
   }.
 
+
+Record StrongBisimulationForProgram
+       (lts1 lts2 : LTS)
+       (compilation_of: forall T, Prog lts1 T -> Prog lts2 T -> Prop)
+       (refines_to: State lts1 -> State lts2 -> Prop)
+       (oracle_refines_to: forall T, State lts1 -> Prog lts2 T -> Oracle lts1 -> Oracle lts2 -> Prop)
+       {T} (p2: Prog lts2 T)
+  :=
+  {
+    strong_bisimulation_for_program_correct:
+      (forall p1 s1 s2 o1 o2,
+          
+          refines_to s1 s2 ->
+          compilation_of T p1 p2 ->
+          oracle_refines_to T s1 p2 o1 o2 ->
+          
+          (forall s1',
+              (exec lts1) T o1 s1 p1 s1' ->
+              exists s2',
+                (exec lts2) T o2 s2 p2 s2' /\
+                result_same s1' s2' /\
+                refines_to (extract_state s1') (extract_state s2') /\
+                (forall def, extract_ret def s1' = extract_ret def s2')) /\
+          (forall s2',
+              (exec lts2) T o2 s2 p2 s2' ->
+              exists s1',
+                (exec lts1) T o1 s1 p1 s1' /\
+                result_same s1' s2' /\
+                refines_to (extract_state s1') (extract_state s2') /\
+                (forall def, extract_ret def s1' = extract_ret def s2')))
+  }.
+
+Record StrongBisimulation
+       (lts1 lts2 : LTS)
+       (compilation_of: forall T, Prog lts1 T -> Prog lts2 T -> Prop)
+       (refines_to: State lts1 -> State lts2 -> Prop)
+       (oracle_refines_to: forall T, State lts1 -> Prog lts2 T -> Oracle lts1 -> Oracle lts2 -> Prop)
+  :=
+  {
+    strong_bisimulation_correct:
+      (forall T p1 (p2: Prog lts2 T) s1 s2 o1 o2,
+          
+          refines_to s1 s2 ->
+          compilation_of T p1 p2 ->
+          oracle_refines_to T s1 p2 o1 o2 ->
+          
+          (forall s1',
+              (exec lts1) T o1 s1 p1 s1' ->
+              exists s2',
+                (exec lts2) T o2 s2 p2 s2' /\
+                result_same s1' s2' /\
+                refines_to (extract_state s1') (extract_state s2') /\
+                (forall def, extract_ret def s1' = extract_ret def s2')) /\
+          (forall s2',
+              (exec lts2) T o2 s2 p2 s2' ->
+              exists s1',
+                (exec lts1) T o1 s1 p1 s1' /\
+                result_same s1' s2' /\
+                refines_to (extract_state s1') (extract_state s2') /\
+                (forall def, extract_ret def s1' = extract_ret def s2')))
+  }.
+
+Lemma bisimulation_restrict_state:
+  forall low high
+
+    refines_to
+    compilation_of
+    oracle_refines_to
+
+    valid_state_h
+    valid_prog_h,
+    
+  StrongBisimulation
+      low
+      high
+      compilation_of
+      refines_to
+      oracle_refines_to ->
+
+  exec_compiled_preserves_validity
+    low
+    high
+    compilation_of                               
+    (refines_to_valid
+       refines_to
+       valid_state_h) ->
+
+  exec_preserves_validity high valid_state_h ->
+  
+  StrongBisimulationForValidStates
+      low
+      high
+      (refines_to_valid
+         refines_to
+         valid_state_h)
+      (compiles_to_valid
+         valid_prog_h
+         compilation_of)
+      valid_state_h
+      valid_prog_h
+      compilation_of
+      refines_to
+      oracle_refines_to.
+Proof.
+  intros.
+  destruct H.
+  constructor; intros.
+  edestruct strong_bisimulation_correct0; eauto.
+  split; intros.
+  edestruct H6; eauto; cleanup.
+  eexists; intuition (eauto).
+
+  edestruct H7; eauto; cleanup.
+  eexists; intuition (eauto).
+Qed.
+
+
+Lemma bisimulation_restrict_prog:
+  forall low high
+
+    refines_to
+    compilation_of
+    oracle_refines_to,
+    
+    (forall T (p: Prog high T),
+      StrongBisimulationForProgram
+      low
+      high
+      compilation_of
+      refines_to
+      oracle_refines_to
+      p) ->
+  
+  StrongBisimulation
+      low
+      high
+      compilation_of
+      refines_to
+      oracle_refines_to.
+Proof.
+  intros.
+  constructor; intros.
+  specialize (H T p2).
+  destruct H.
+  edestruct strong_bisimulation_for_program_correct0; eauto.
+Qed.
+
 Theorem transfer_high_to_low :
   forall low high
 
@@ -160,7 +312,7 @@ Theorem transfer_high_to_low :
       valid_prog_h
       related_states_h ->
     
-    StrongBisimulation
+    StrongBisimulationForValidStates
       low
       high
       (refines_to_valid
@@ -187,10 +339,10 @@ Theorem transfer_high_to_low :
          refines_to
          related_states_h).
 Proof.
-  unfold refines_to_related, compiles_to_valid, oracle_refines_to_valid; intros.
+  unfold refines_to_related, compiles_to_valid; intros.
   destruct H, H0.
   rename self_simulation_correct0 into self_simulation_correct.
-  rename strong_bisimulation_correct0 into strong_bisimulation_correct.
+  rename strong_bisimulation_for_valid_states_correct0 into strong_bisimulation_correct.
   
   eapply Build_SelfSimulation;  intros; cleanup.
 
@@ -298,7 +450,7 @@ Lemma bisimulation_weaken_valid_prog:
 
     (forall (T: Type) (p: Prog high T), valid_prog_h1 T p -> valid_prog_h2 T p) ->
     
-  StrongBisimulation
+    StrongBisimulationForValidStates
       low
       high
       (refines_to_valid
@@ -313,7 +465,7 @@ Lemma bisimulation_weaken_valid_prog:
       refines_to
       oracle_refines_to ->
 
-  StrongBisimulation
+    StrongBisimulationForValidStates
       low
       high
       (refines_to_valid
@@ -331,229 +483,7 @@ Proof.
   intros.
   destruct H0.
   constructor; intros.
-  eapply strong_bisimulation_correct0; eauto.
+  eapply strong_bisimulation_for_valid_states_correct0; eauto.
   unfold compiles_to_valid in *; cleanup.
   eexists; eauto.
 Qed.
-
-
-(*
-Definition oracle_refines_to_valid
-           {State1 State2 Oracle1 Oracle2: Type} {Op1 Op2: Type -> Type}
-           (oracle_refines_to: forall T, State1 -> Op2 T -> Oracle1 -> Oracle2 -> Prop)
-           (refines_to: State1 -> State2 -> Prop)
-           (compilation_of: forall T, Op1 T -> Op2 T -> Prop)
-           (valid_oracle2: forall T, Oracle2 -> State2 -> Op2 T -> Prop)
-           T (o1: Oracle1) (st1: State1) (p1: Op1 T) :=
-  forall st2 p2,
-    refines_to st1 st2 ->
-    compilation_of T p1 p2 ->
-    exists o2, oracle_refines_to T st1 p2 o1 o2 /\
-    valid_oracle2 T o2 st2 p2.
-
-
-
-Definition oracle_equal_with_respect_to
-           {State Oracle1 Oracle2: Type} {Op: Type -> Type}
-           (related: State -> State -> Prop)
-           (oracle_refines_to: forall T, State -> Op T -> Oracle1 -> Oracle2 -> Prop):=
-  forall T o1 o2 o2' st1 st2 p,
-    oracle_refines_to T st1 p o1 o2 ->
-    oracle_refines_to T st2 p o1 o2' ->
-    related st1 st2 ->
-    o2 = o2'.
-
-
-Record SelfSimulation (lts: LTS)
-       (valid_state: State lts -> Prop)
-       (valid_op: forall T, Prog lts T -> Prop)
-       (valid_oracle: forall T, list (Token lts) -> State lts -> Prog lts T -> Prop)
-       (R: State lts -> State lts -> Prop) :=
-  {
-    self_simulation_correct:
-      forall T o p s1 s1' s2,
-        valid_state s1 ->
-        valid_state s2 ->
-        valid_op T p ->
-        valid_oracle T o s1 p ->
-        valid_oracle T o s2 p ->
-        (exec lts) T o s1 p s1' ->
-        R s1 s2 ->
-        exists s2',
-          (exec lts) T o s2 p s2' /\
-          result_same s1' s2' /\
-          R (extract_state s1') (extract_state s2') /\
-          (forall def, extract_ret def s1' = extract_ret def s2') /\
-          valid_state (extract_state s1') /\
-          valid_state (extract_state s2') ;
-  }.
-
-Record StrongBisimulation
-       (lts1 lts2 : LTS)
-       (valid_state1 : State lts1 -> Prop)
-       (valid_op1: forall T, Prog lts1 T -> Prop)
-       (valid_state2 : State lts2 -> Prop)
-       (valid_op2: forall T, Prog lts2 T -> Prop)
-       (compilation_of: forall T, Prog lts1 T -> Prog lts2 T -> Prop)
-       (refines_to: State lts1 -> State lts2 -> Prop)
-       (oracle_refines_to: forall T, State lts1 -> Prog lts2 T -> list (Token lts1) -> list (Token lts2) -> Prop)
-  :=
-  {
-    strong_bisimulation_correct:
-      (forall T p1 p2 o1 o2 s1 s2,
-          valid_state1 s1 ->
-          valid_op1 T p1 ->
-          
-          valid_state2 s2 ->
-          valid_op2 T p2 ->
-          
-          refines_to s1 s2 ->
-          compilation_of T p1 p2 ->
-          
-          oracle_refines_to T s1 p2 o1 o2 ->
-          
-          (forall s1',
-              (exec lts1) T o1 s1 p1 s1' ->
-              exists s2',
-                (exec lts2) T o2 s2 p2 s2' /\
-                result_same s1' s2' /\
-                refines_to (extract_state s1') (extract_state s2') /\
-                (forall def, extract_ret def s1' = extract_ret def s2') /\
-                valid_state1 (extract_state s1') /\ valid_state2 (extract_state s2')) /\
-          (forall s2',
-              (exec lts2) T o2 s2 p2 s2' ->
-              exists s1',
-                (exec lts1) T o1 s1 p1 s1' /\
-                result_same s1' s2' /\
-                refines_to (extract_state s1') (extract_state s2') /\
-                (forall def, extract_ret def s1' = extract_ret def s2')/\
-                valid_state1 (extract_state s1') /\ valid_state2 (extract_state s2')))
-  }.
-
-Theorem transfer_high_to_low :
-  forall low high
-
-    eqv_h
-    refines_to
-    compilation_of
-    oracle_refines_to
-
-    valid_h
-    valid_op_h
-    valid_oracle_h,
-    
-    SelfSimulation
-      high
-      valid_h
-      valid_op_h
-      valid_oracle_h
-      eqv_h ->
-    
-    StrongBisimulation
-      low
-      high
-      (refines_to_valid
-         refines_to
-         valid_h)
-      (compiles_to_valid
-         valid_op_h
-         compilation_of)
-      valid_h
-      valid_op_h
-      compilation_of
-      refines_to
-      oracle_refines_to ->
-
-    oracle_equal_with_respect_to
-      (refines_to_related
-         refines_to
-         eqv_h)
-      oracle_refines_to ->
-    
-    SelfSimulation
-      low
-      (refines_to_valid
-         refines_to
-         valid_h)
-      (compiles_to_valid
-         valid_op_h
-         compilation_of)
-      (oracle_refines_to_valid
-         oracle_refines_to
-         refines_to
-         compilation_of
-         valid_oracle_h)
-      (refines_to_related
-         refines_to
-         eqv_h).
-Proof.
-  unfold refines_to_related, compiles_to_valid, oracle_refines_to_valid, oracle_equal_with_respect_to; intros.
-  destruct H, H0.
-  rename self_simulation_correct0 into self_simulation_correct.
-  rename strong_bisimulation_correct0 into strong_bisimulation_correct.
-  rename H1 into oracle_equal.
-  
-  eapply Build_SelfSimulation;  intros; cleanup.
-  repeat match goal with
-    | [H: forall (_ : State high) (_ : Prog high _), _ |- _] =>
-      edestruct H; eauto; cleanup; clear H
-         end.
-  
-  match goal with
-  | [H: oracle_refines_to _ _ _ _ _,
-     H0: oracle_refines_to _ _ _ _ _ |- _] =>
-    eapply_fresh oracle_equal in H;
-      try apply H0; eauto; cleanup
-  end.
-  
-  match goal with
-  | [H: refines_to s1 _ |- _] =>
-    eapply_fresh strong_bisimulation_correct in H; eauto; cleanup
-  end.
-
-  match goal with
-    | [H: forall _, exec low _ _ _ _ _ -> _,
-       H0: exec low _ _ _ _ _,
-       H1: forall _, exec high _ _ _ _ _ -> _ |- _] =>
-      eapply H in H0; cleanup; clear H H1
-  end.
-
-  match goal with
-  | [H: refines_to_valid _ _ ?s,
-     H0: refines_to ?s _,
-     H1: refines_to_valid _ _ ?t,
-     H2: refines_to ?t _ |- _] =>
-    eapply_fresh H in H0;
-      eapply_fresh H1 in H2; cleanup
-  end.
-
-  match goal with
-    | [H: exec high _ _ _ _ _ |- _] =>
-      eapply self_simulation_correct in H; eauto; cleanup
-  end.
-
-  match goal with
-  | [H: exec high _ _ ?x2 _ _,
-     H0: refines_to ?s1 ?x1,
-     H1: refines_to ?s2 ?x2,      
-     H2: refines_to_valid _ _ ?s2 |- _] =>
-      eapply strong_bisimulation_correct in H1; eauto; cleanup
-  end.
-  
-  match goal with
-    | [H: forall _, exec low _ _ _ _ _ -> _,
-       H0: exec high _ _ _ _ _,
-       H1: forall _, exec high _ _ _ _ _ -> _ |- _] =>
-      eapply H1 in H0; cleanup; clear H H1
-  end.
-
-  eexists; intuition eauto.
-  do 2 (eapply result_same_transitive; eauto).
-  apply result_same_symmetric; auto.
-  
-  repeat match goal with
-  | [H: forall _, extract_ret _ ?a = _ |- extract_ret _ ?a = _] =>
-    rewrite H; auto
-  end.
-Qed.
-*)
