src/BlockAllocatorDefinitions.v
@@ -1,0 +1,113 @@
+Require Import Primitives Omega Disk ListUtils.
+Close Scope pred_scope.
+
+Axiom block_size: nat.
+Axiom block_size_eq: block_size = 64.
+
+Definition valid_bitlist l := length l = block_size /\ (forall i, In i l -> i < 2).
+Record bitlist :=
+  {
+   bits : list nat;                
+   valid : valid_bitlist bits
+  }.
+
+Fixpoint get_first_zero l :=
+  match l with
+  | nil => 0
+  | hd::tl =>
+    match hd with
+    | O => 0
+    | _ => S (get_first_zero tl)
+    end
+  end.
+
+Theorem upd_valid_zero:
+  forall i l,
+    valid_bitlist l ->
+    valid_bitlist (updN l i 0).
+Proof. Admitted.
+
+Theorem upd_valid_one:
+  forall i l,
+    valid_bitlist l ->
+    valid_bitlist (updN l i 1).
+Proof. Admitted.
+
+Axiom value_to_bits: value -> bitlist.
+Axiom bits_to_value: bitlist -> value.
+Axiom value_to_bits_to_value : forall v, bits_to_value (value_to_bits v) = v.
+Axiom bits_to_value_to_bits : forall l, value_to_bits (bits_to_value l) = l.                                                                   
+Open Scope pred_scope.
+
+Fixpoint ptsto_bits' (dh: disk value) bits n : @pred addr addr_dec (set value) :=
+  match bits with
+  | nil =>
+    emp
+  | b::l =>
+    (exists vs,
+    (S n) |-> vs *
+    match b with
+    | 0 => [[ dh n = None ]]
+    | 1 => [[ dh n = Some (fst vs) ]]
+    | _ => [[ False ]]
+    end) *
+    ptsto_bits' dh l (S n)
+  end.
+      
+Definition ptsto_bits dh bits := ptsto_bits' dh bits 0.
+
+Definition rep (dh: disk value) : @pred addr addr_dec (set value) :=
+  (exists bitmap bl,
+    let bits := bits (value_to_bits bitmap) in
+    0 |-> (bitmap, bl) * ptsto_bits dh bits * [[ forall i, i >= block_size -> dh i = None ]])%pred.
+
+Definition alloc (v': value) : prog (option addr) :=
+  v <- Read 0;
+  let bits := bits (value_to_bits v) in
+  let valid := valid (value_to_bits v) in
+  let index := get_first_zero bits in
+  
+  if lt_dec index block_size then
+    _ <- Write (S index) v';
+    _ <- Write 0 (bits_to_value (Build_bitlist (updN bits index 1) (upd_valid_one index bits valid)));
+    Ret (Some index)
+  else
+    Ret None.
+
+Definition read a : prog (option value) :=
+  v <- Read 0;
+  let bits := bits (value_to_bits v) in
+  if lt_dec a block_size then
+    if addr_dec (nth a bits 0) 1 then
+      h <- Read (S a);
+      Ret (Some h)
+    else
+      Ret None
+  else
+    Ret None.
+
+Definition write a v' : prog (option unit) :=
+  v <- Read 0;
+  let bits := bits (value_to_bits v) in
+  if lt_dec a block_size then
+    if addr_dec (nth a bits 0) 1 then
+      _ <- Write (S a) v';
+      Ret (Some tt)
+    else
+      Ret None
+  else
+    Ret None.
+
+Definition free a : prog unit :=
+  v <- Read 0;
+  let bits := bits (value_to_bits v) in
+  let valid := valid (value_to_bits v) in
+  if lt_dec a block_size then
+    if addr_dec (nth a bits 0) 1 then
+      Write 0 (bits_to_value (Build_bitlist (updN bits a 0) (upd_valid_zero a bits valid)))
+    else
+      Ret tt
+  else
+    Ret tt.
+
+Hint Extern 0 (okToUnify (rep _) (rep _)) => constructor : okToUnify.
