src/BlockAllocatorFacts.v
@@ -1,0 +1,393 @@
+Require Import Primitives Omega Disk FunctionalExtensionality.
+Require Import BlockAllocatorDefinitions ListUtils.
+
+
+Lemma delete_eq:
+  forall A AEQ V (m: @mem A AEQ V) a,
+    delete m a a = None.
+Proof.
+  intros; unfold delete; simpl.
+  destruct (AEQ a a); intuition.
+Qed.
+
+Lemma delete_ne:
+  forall A AEQ V (m: @mem A AEQ V) a a',
+    a <> a' ->
+    delete m a a' = m a'.
+Proof.
+  intros; unfold delete; simpl.
+  destruct (AEQ a' a); subst; intuition.
+Qed.
+        
+
+Lemma star_split:
+    forall (AT : Type) (AEQ : EqDec AT) (V : Type)
+      (p q : @pred AT AEQ V) (m : @mem AT AEQ V),
+      (p * q)%pred m ->
+      (exists m1 m2, mem_disjoint m1 m2 /\ p m1 /\ q m2 /\ mem_union m1 m2 = m)%type.
+  Proof.
+    intros; unfold sep_star in *; rewrite sep_star_is in *;
+      destruct H; cleanup; eauto.
+    do 2 eexists; intuition eauto.
+  Qed.
+
+Theorem hoare_triple_pre_ex':
+  forall T V (p: prog T) pre post crash,
+  (forall (v: V), hoare_triple (fun a d => pre v a d) p post crash) ->
+  hoare_triple (fun a d => (exists (v: V), pre v a) d) p post crash.
+Proof.
+  unfold hoare_triple; intros.
+  destruct_lift H0; cleanup.
+  eapply H; eauto.
+Qed.
+
+Theorem hoare_triple_pre_ex:
+  forall T V (p: prog T) pre post crash F P,
+  (forall (v: V), hoare_triple (fun a d => ((F * (fun d' => pre v a d')) * [[ P a d ]]) d) p post crash) ->
+  hoare_triple (fun a d => ((F * (fun d' => (exists (v: V), pre v a) d')) * [[ P a d ]]) d) p post crash.
+Proof.
+  intros.
+  eapply hoare_triple_strengthen_pre.
+  apply hoare_triple_pre_ex'.
+  instantiate (1:= fun v a d => ((F * (pre v a)) * [[ P a d ]]) d).
+  simpl; eauto.
+  intros; norm.
+  unfold stars; simpl.
+  intros mx Hmx; simpl in *.
+  destruct_lift Hmx.
+  destruct_lift H0.
+  destruct_lift H0.
+  exists dummy.
+  pred_apply' H0; norm.
+  cancel.
+  all: eauto.
+Qed.
+
+Lemma upd_eq':
+  forall (A V : Type) (AEQ : EqDec A) (m : mem) (a : A) (v : V),
+    @upd _ _ AEQ m a v a = Some v.
+Proof.
+  intros; apply upd_eq; eauto.
+Qed.
+
+Lemma ptsto_bits'_app_split:
+  forall l1 l2 n dh,
+    ptsto_bits' dh (l1++l2) n =p=>
+    (ptsto_bits' dh l1 n * ptsto_bits' dh l2 (n + length l1))%pred.
+Proof.
+  unfold ptsto_bits; induction l1;
+    simpl; intros; eauto.
+  rewrite Nat.add_0_r; cancel.
+  rewrite IHl1; cancel.
+  rewrite Nat.add_succ_r; eauto.
+Qed.
+
+Lemma ptsto_bits'_app_merge:
+  forall l1 l2 n dh,
+    (ptsto_bits' dh l1 n * ptsto_bits' dh l2 (n + length l1))%pred =p=>
+     ptsto_bits' dh (l1++l2) n.
+Proof.
+  unfold ptsto_bits; induction l1;
+    simpl; intros; eauto.
+  rewrite Nat.add_0_r; cancel.
+  rewrite <- IHl1; cancel.
+  rewrite Nat.add_succ_r; eauto.
+Qed.
+
+Lemma ptsto_bits'_inbound:
+  forall l n dh a F d,
+    a < length l + n ->
+    a >= n ->
+    (F * ptsto_bits' dh l n)%pred d ->
+    (exists vs, d (S a) = Some vs /\
+           (nth (a - n) l 0 = 0 -> dh a = None) /\
+           (nth (a - n) l 0 = 1 -> dh a = Some (fst vs)) /\
+           (nth (a - n) l 0 < 2))%type.
+Proof.
+   eapply (rev_ind
+             (fun l =>
+                forall (n : nat) (dh : disk value) (a : nat) (F : pred) (d : mem),
+  a < length l + n ->
+  a >= n ->
+  (F ✶ ptsto_bits' dh l n) d ->
+  exists vs : set value,
+    (d (S a) = Some vs /\
+     (nth (a - n) l 0 = 0 -> dh a = None) /\
+     (nth (a - n) l 0 = 1 -> dh a = Some (fst vs)) /\
+     (nth (a - n) l 0 < 2))%type
+));
+     simpl; intros.
+   omega.
+
+   rewrite app_length in *; simpl in *.
+   rewrite ptsto_bits'_app_split in *; simpl in *.
+   destruct (addr_dec a (n + length l)); subst.
+   - rewrite minus_plus.
+     rewrite app_nth2; try omega.
+     rewrite Nat.sub_diag; simpl.
+     destruct_lifts.
+     eexists; split.
+     eapply ptsto_valid; pred_apply; cancel.
+     intuition; subst;
+       destruct_lifts; eauto.
+     destruct x; eauto.
+     destruct x; eauto.
+     destruct_lifts; tauto.
+   - destruct_lifts.
+     rewrite app_nth1; try omega.
+     eapply H; eauto.
+     omega.
+     pred_apply' H2; cancel.
+Qed.
+
+Lemma septract_sep_star_extract :
+  forall AT AEQ V (p q: @pred AT AEQ V),
+    q =p=> (exists F, F * p) ->
+    q =p=> (p --* q) * p.
+Proof.
+  intros.
+  intros m Hm.
+  eapply_fresh H in Hm.
+  destruct_lift Hx.
+  apply star_split in H0; cleanup.
+  
+  unfold sep_star; rewrite sep_star_is.
+  unfold sep_star_impl.
+  unfold septract.
+  do 2 eexists; intuition.
+  eexists; intuition eauto.
+Qed.
+
+Lemma septract_sep_star_extract' :
+  forall AT AEQ V (p q: @pred AT AEQ V) m,
+    (exists F, F * p)%pred m ->
+    q m ->
+    ((p --* q) * p)%pred m.
+Proof.
+  intros.
+  destruct_lift H.
+  apply star_split in H; cleanup.
+  
+  unfold sep_star; rewrite sep_star_is.
+  unfold sep_star_impl.
+  unfold septract.
+  do 2 eexists; intuition.
+  eexists; intuition eauto.
+Qed.
+
+Lemma septract_sep_star_merge :
+  forall AT AEQ V (p q: @pred AT AEQ V),
+    (forall m m', p m -> p m' -> m = m') ->
+    (p --* q) * p =p=> q.
+Proof.
+  unfold septract; intros.
+  intros m Hm.
+  apply star_split in Hm; cleanup.
+  erewrite (H x0); eauto.
+Qed.
+
+Lemma ptsto_bits'_extract:
+  forall l n dh a,
+    a < length l + n ->
+    a >= n ->
+    ptsto_bits' dh l n =p=> exists vs, (((S a |-> vs) --* ptsto_bits' dh l n) * (S a |-> vs)).
+Proof.
+  intros.
+  intros m Hm.
+  edestruct ptsto_bits'_inbound; eauto.
+  pred_apply' Hm; eassign dh; cancel.
+  cleanup.
+  exists x.
+  
+  eapply septract_sep_star_extract' in Hm; eauto.
+  exists (diskIs (mem_except m (S a))).
+  eapply diskIs_extract' in H1.
+  assert (A: diskIs m m).
+  unfold diskIs; eauto.
+  apply H1 in A; eauto.
+Qed.
+
+Lemma ptsto_bits'_merge:
+  forall l n dh a vs,
+    ((S a |-> vs) --* ptsto_bits' dh l n) * (S a |-> vs) =p=> ptsto_bits' dh l n.
+Proof.
+  intros.
+  unfold septract; intros.
+  intros m Hm.
+  apply star_split in Hm; cleanup.
+  destruct_lift H3.
+  eapply ptsto_complete in H3; eauto; subst; eauto.
+Qed.
+
+Lemma rep_eq:
+  forall d s1 s2 F F',
+    (F * rep s1)%pred d ->
+    (F' * rep s2)%pred d ->
+    s1 = s2.
+Proof.
+  intros.
+  extensionality k.
+  unfold rep in *; simpl in *.
+  
+  destruct_lift H; destruct_lift H0.
+  assert_fresh (d 0 = Some (dummy,dummy0)).
+  eapply ptsto_valid'; pred_apply' H; cancel.
+  assert_fresh (d 0 = Some (dummy1,dummy2)).
+  eapply ptsto_valid'; pred_apply' H0; cancel.
+  cleanup.
+
+  destruct (lt_dec k block_size).
+  
+  unfold ptsto_bits in *.
+  eapply (@ptsto_bits'_inbound _ _ _ k) in H; try omega; cleanup.
+  eapply (@ptsto_bits'_inbound _ _ _ k) in H0; try omega; cleanup.
+  rewrite Nat.sub_0_r in *.
+  
+  destruct_fresh (nth k (bits (value_to_bits dummy1)) 0).
+  rewrite H1, H6; eauto.
+  destruct n; try omega.
+  rewrite H2, H7; eauto.
+  destruct (value_to_bits dummy1); simpl in *.
+  unfold valid_bitlist in *; cleanup.
+  omega.
+  destruct (value_to_bits dummy1); simpl in *.
+  unfold valid_bitlist in *; cleanup.
+  omega.
+  erewrite H4, H5; eauto; omega.   
+Qed.      
+
+Lemma ptsto_bits'_update_oob:
+  forall l n dh a v,
+    a >= length l + n ->
+    ptsto_bits' dh l n ⇨⇨ ptsto_bits' (upd dh a v) l n.
+Proof.
+  eapply (rev_ind
+    (fun l =>
+       forall n dh a v,
+    a >= length l + n ->
+    ptsto_bits' dh l n ⇨⇨ ptsto_bits' (upd dh a v) l n));
+    simpl in *; intros.
+  cancel.
+  rewrite app_length in *; simpl in *.
+  rewrite ptsto_bits'_app_split; simpl in *.
+  rewrite <- ptsto_bits'_app_merge; simpl.
+  rewrite <- H; try omega.
+  cancel.
+  rewrite upd_ne; eauto.
+  omega.
+Qed.
+  
+ Lemma ptsto_bits'_update_apply:
+   forall l n a v vs dh m F,
+     a < length l + n ->
+     a >= n ->
+     m (S a) = Some vs ->
+     (F * ptsto_bits' dh l n)%pred m ->
+     (F * ptsto_bits' (upd dh a v) (updN l (a - n) 1) n)%pred (upd m (S a) (v, fst vs::snd vs)).
+ Proof.
+   eapply (rev_ind
+    (fun l =>
+       forall n a v vs dh m F,
+         a < length l + n ->
+         a >= n ->
+         m (S a) = Some vs ->
+         (F * ptsto_bits' dh l n)%pred m ->
+         (F * ptsto_bits' (upd dh a v) (updN l (a - n) 1) n)%pred (upd m (S a) (v, fst vs::snd vs))));
+     simpl in *; intros.
+   omega.
+   rewrite app_length in *; simpl in *.
+   rewrite ptsto_bits'_app_split in H3; simpl in *.
+   destruct (addr_dec a (length l + n)); subst.
+   -
+     rewrite Nat.add_sub.
+     rewrite updN_app_tail; simpl.
+     rewrite <- ptsto_bits'_app_merge; simpl.
+     destruct_lift H3.
+     eapply pimpl_apply.
+     2: rewrite Nat.add_comm;
+       eapply ptsto_upd;
+       pred_apply; cancel.
+     cancel.
+     erewrite <- ptsto_bits'_update_oob.
+     cancel.
+     destruct x; cancel.
+     destruct x; cancel.
+     eauto.
+     rewrite Nat.add_comm, upd_eq'; eauto.
+   -
+     rewrite updN_app1; try omega.
+     rewrite <- ptsto_bits'_app_merge.
+     simpl.
+     rewrite length_updN.
+     eapply pimpl_apply.
+     2: {
+       eapply H; eauto.
+       omega.
+       eassign dh;
+         eassign (F
+        ✶  ((exists vs : value * list value,
+                 S (n + length l) |-> vs
+                 ✶ match x with
+                   | 0 => ⟦⟦ dh (n + length l) = None ⟧⟧
+                   | 1 => ⟦⟦ dh (n + length l) = Some (fst vs) ⟧⟧
+                   | S (S _) => ⟦⟦ False ⟧⟧
+                   end) ✶ emp)).
+       pred_apply; cancel.
+     }
+     rewrite upd_ne; try omega.
+     cancel.
+ Qed.
+
+ Lemma ptsto_bits'_update_septract:
+   forall l n a v vs dh,
+     a < length l + n ->
+     a >= n ->
+     S a |-> vs --* ptsto_bits' dh l n =p=>
+     S a |-> (v, fst vs::snd vs) --* ptsto_bits' (upd dh a v) (updN l (a - n) 1) n.
+ Proof.
+
+   
+   intros.
+   unfold septract, pimpl; intros.
+   cleanup.
+
+   unfold emp in *; simpl in *.
+   assert (A: x (S a) = Some vs).
+   eapply ptsto_valid'.
+   pred_apply' H2; cancel.
+   exists (upd x (S a) (v, fst vs :: snd vs)).
+   intuition.
+   apply mem_disjoint_comm.
+   eapply mem_disjoint_upd; eauto.
+   apply mem_disjoint_comm; eauto.
+   eapply emp_star.
+   eapply ptsto_upd'; pred_apply; cancel.
+   rewrite mem_union_comm.
+   rewrite mem_union_upd.
+   apply emp_star.
+   eapply ptsto_bits'_update_apply; eauto.
+
+   apply mem_disjoint_comm in H1.
+   eapply mem_union_addr in A; eauto.
+   rewrite mem_union_comm; eauto.
+   pred_apply; cancel.
+   apply mem_disjoint_comm in H1; eauto.
+   apply mem_disjoint_comm.
+   eapply mem_disjoint_upd; eauto.
+   apply mem_disjoint_comm; eauto.
+ Qed.
+   
+
+ Lemma ptsto_bits'_update:
+   forall l n a v vs dh,
+     a < length l + n ->
+     a >= n ->
+      S a |-> vs --* ptsto_bits' dh l n
+  ✶ S a |-> (v, fst vs :: snd vs)
+  ⇨⇨ ptsto_bits' (upd dh a v)
+  (updN l (a-n) 1) n.
+ Proof.
+   intros.
+   rewrite ptsto_bits'_update_septract; eauto.
+   rewrite ptsto_bits'_merge; eauto.
+ Qed.
