src/BlockAllocatorSpecs.v
@@ -1,0 +1,1086 @@
+Require Import Primitives Omega Disk.
+Require Import BlockAllocatorDefinitions BlockAllocatorFacts.
+Require Import Layer2 Layer1to2RefinementDefinitions.
+
+Arguments oracle_ok T p o s : simpl never.
+
+
+Theorem alloc_ok:
+  forall dh v,
+  << o >>
+   (rep dh)
+   (alloc v)
+  << d, r >>
+   (exists dh',
+    rep dh' *
+     [[(r = None /\ dh' = dh /\ oracle_refines_to _ d (Alloc v) o (DiskFull::nil)) \/
+       (exists a, r = Some a /\ dh a = None /\ dh' = upd dh a v /\ oracle_refines_to _ d (Alloc v) o (BlockNum a::nil))%type]])
+   (exists dh',
+    rep dh' *
+     [[(dh' = dh /\ oracle_refines_to _ d (Alloc v) o (Crash1::nil)) \/
+       (exists a, dh a = None /\ dh' = upd dh a v /\ oracle_refines_to _ d (Alloc v) o (CrashAlloc a::nil) )%type]]).
+Proof. Admitted. (*
+  unfold alloc; intros dh v.
+  unfold rep.
+  repeat (apply extract_exists; intros).
+  eapply crash_weaken.
+  eapply bind_ok.  
+  eapply pre_strengthen.
+  eapply add_frame.
+  apply read_ok.
+  eassign (ptsto_bits dh (bits (value_to_bits v0)) *
+           [[ forall i : nat, i >= block_size -> dh i = None ]]).
+  cancel.
+  simpl; intros; cancel.
+ 
+  intros; destruct_lifts.
+  destruct (lt_dec (get_first_zero (bits (value_to_bits v0))) block_size); simpl in *.
+  {
+    eapply hoare_triple_strengthen_pre.
+    2: {
+      unfold ptsto_bits.
+      intros.
+      
+      instantiate (1:= (fun o0 => (fun d0 => ( F2 * (exists vs, (S (get_first_zero (bits (value_to_bits v0)))|-> vs) * 0 |-> (v0, v1) * ((S (get_first_zero (bits (value_to_bits v0)))|-> vs) --* ptsto_bits' dh (bits (value_to_bits v0)) 0))
+    ✶ ⟦⟦ oracle_ok
+           (_ <- Write (S (get_first_zero (bits (value_to_bits v0)))) v;
+            _ <-
+            Write 0
+              (bits_to_value
+                 {|
+                 bits := ListUtils.updN (bits (value_to_bits v0)) (get_first_zero (bits (value_to_bits v0))) 1;
+                 valid := upd_valid_one (get_first_zero (bits (value_to_bits v0))) (bits (value_to_bits v0))
+                            (valid (value_to_bits v0)) |}); Ret (Some (get_first_zero (bits (value_to_bits v0)))))
+           o0 d0 ⟧⟧) d0)%pred)).
+      simpl.
+      intros m Hm; simpl in *;
+        pred_apply; clear Hm.
+      erewrite (ptsto_bits'_extract (bits (value_to_bits v0))) at 1.
+      norml.
+      cancel.
+      eauto.
+      rewrite Nat.add_0_r.
+      destruct (value_to_bits v0); simpl in *.
+      destruct valid.
+      rewrite H2; eauto.
+      omega.
+    }    
+    repeat (apply extract_exists; intros).
+    destruct v2.
+    eapply crash_weaken.    
+    eapply pre_strengthen.
+    eapply bind_ok.
+    eapply add_frame.
+    apply write_ok.
+
+    simpl; intros; eauto.
+
+    simpl; intros.
+    eapply hoare_triple_strengthen_pre.
+    eapply crash_weaken.
+    eapply bind_ok.
+    eapply add_frame.
+    eapply write_ok.
+
+    simpl; intros; eauto.
+
+    simpl in *; intros.
+    eapply hoare_triple_strengthen_pre.
+    eapply crash_weaken.
+    eapply post_weaken.
+    eapply add_frame.
+    apply ret_ok.
+
+    - (* post *)
+      simpl; intros.
+      shelve.
+    - eauto.
+    - simpl; intros.
+      cancel.
+      intros m Hm; simpl in *;
+        pred_apply; clear Hm.
+      shelve.
+    - eauto.
+    - simpl; intros; cancel.
+      intros m Hm; simpl in *;
+        pred_apply; clear Hm.
+      cancel.
+      shelve.
+    - cancel.
+    - instantiate (1:= 
+        (exists dh',
+            rep dh' *
+            [[(dh' = dh) \/
+              (exists h, dh' = upd dh h v)%type]])).
+      unfold rep.
+      unfold ptsto_bits.
+      shelve.
+  }
+  {
+    simpl in *; intros.
+    eapply hoare_triple_strengthen_pre.
+    eapply crash_weaken.
+    eapply post_weaken.
+    eapply add_frame.
+    apply ret_ok.
+
+    - destruct_lift H.
+      simpl; safecancel.
+      eauto.
+      eauto.
+    - unfold rep; simpl; cancel.
+    - intros.
+      intros m Hm; simpl in *;
+        pred_apply; clear Hm.
+      simpl; cancel.
+  }
+  {
+    unfold rep; cancel.
+    cleanup.
+    right.
+    do 2 eexists; eauto.
+  }
+  Unshelve.
+  {
+    safecancel.
+    2: right; eauto.
+    erewrite upd_ne.
+    eauto.
+    omega.
+  }
+  {
+    cancel.
+  }
+  shelve.
+  {
+    rewrite bits_to_value_to_bits; simpl.
+    cancel.
+    unfold ptsto_bits.
+    rewrite ptsto_bits'_update.
+    rewrite Nat.sub_0_r; eauto.
+    destruct (value_to_bits v0); simpl in *.
+    destruct valid.
+    rewrite e; eauto.
+    omega.
+    omega.
+  }
+  {
+    safecancel; eauto.
+    rewrite sep_star_comm.
+    apply ptsto_bits'_merge.
+        
+    rewrite bits_to_value_to_bits; simpl.
+    unfold ptsto_bits.
+    
+    admit.
+    erewrite upd_ne.
+    eauto.
+    omega.
+  }  
+Admitted.
+*)
+Theorem read_ok:
+  forall a dh,
+  << o >>
+   (rep dh)
+   (read a)
+  << d, r >>
+  (rep dh * [[ oracle_refines_to _ d (Read a) o (Cont::nil) ]] *
+   [[(r = None /\ (dh a = None \/ a >= block_size)) \/
+     (exists v, r = Some v /\ dh a = Some v)%type]])
+   (rep dh * [[ oracle_refines_to _ d (Read a) o (Crash1::nil) ]]).
+Proof. Admitted. (*
+  intros.
+  unfold read; simpl.
+
+  unfold rep.
+  repeat (apply hoare_triple_pre_ex; intros).
+  
+  eapply hoare_triple_pimpl;
+    try solve [intros; simpl in *; eauto].
+  eapply hoare_triple_strengthen_pre;
+    [apply read_okay | intros; simpl; cancel].
+
+  simpl. destruct (addr_dec a 1); subst.
+  {
+    intros; simpl.
+    destruct (addr_dec (value_to_nat r) 1); simpl.
+    {
+    eapply hoare_triple_pimpl;
+    try solve [intros; simpl in *; eauto].
+    eapply hoare_triple_strengthen_pre;
+    [apply read_okay | intros; simpl; cancel].
+
+    {
+      intros; simpl.
+      eapply hoare_triple_weaken_post_weak.
+      eapply hoare_triple_weaken_crash_strong.
+      eapply hoare_triple_strengthen_pre.
+      apply ret_okay.
+      
+      intros; simpl in *.
+      destruct_lift H;
+        destruct_lift H0; cleanup;
+          cancel; eauto.
+      
+      intros; simpl in *.
+      destruct_lift H;
+        destruct_lift H0; cleanup;
+          cancel; eauto.
+
+      intros; simpl in *.
+      destruct_lift H;
+        destruct_lift H0;
+        destruct_lift H1;
+        cleanup;
+          cancel; eauto.
+    }
+    intros; simpl in *;
+      destruct_lift H;
+      destruct_lift H0; cleanup;
+        norm; [cancel| intuition (eauto; try omega)].
+    }
+
+    destruct (addr_dec (value_to_nat r) 3); simpl.
+    {
+    eapply hoare_triple_pimpl;
+    try solve [intros; simpl in *; eauto].
+    eapply hoare_triple_strengthen_pre;
+    [apply read_okay | intros; simpl; cancel].
+
+    {
+      intros; simpl.
+      eapply hoare_triple_weaken_post_weak.
+      eapply hoare_triple_weaken_crash_strong.
+      eapply hoare_triple_strengthen_pre.
+      apply ret_okay.
+      
+      intros; simpl in *.
+      destruct_lift H;
+        destruct_lift H0; cleanup;
+          cancel; eauto.
+      
+      intros; simpl in *.
+      destruct_lift H;
+        destruct_lift H0; cleanup;
+          cancel; eauto.
+
+      intros; simpl in *.
+      destruct_lift H;
+        destruct_lift H0;
+        destruct_lift H1;
+        cleanup;
+          cancel; eauto.
+    }
+    intros; simpl in *;
+      destruct_lift H;
+      destruct_lift H0; cleanup;
+        norm; [cancel| intuition (eauto; try omega)].
+    }
+
+      {
+      intros; simpl.
+      eapply hoare_triple_weaken_post_weak.
+      eapply hoare_triple_weaken_crash_strong.
+      eapply hoare_triple_strengthen_pre.
+      apply ret_okay.
+
+      eassign (F * rep dh * ⟦⟦ r = v ⟧⟧).
+      destruct_lift H;
+        cleanup.
+      intros; simpl in *; unfold rep; cancel.
+      
+      unfold rep; intros; simpl in *.
+      destruct_lift H; cleanup.
+      norm; [cancel| intuition (eauto; try omega)].
+      
+
+      intros; simpl in *.
+      unfold rep;
+      destruct_lift H; cleanup;
+      norm; [cancel| intuition (eauto; try omega)].
+      
+      left; split; eauto.
+      left.
+      destruct (addr_dec (value_to_nat v) 0).
+      destruct H8; eauto.
+      destruct (addr_dec (value_to_nat v) 2);
+        destruct H6; eauto.
+      omega.
+    }
+  }
+  
+
+  destruct (addr_dec a 2); subst.
+  {
+    intros; simpl.
+    destruct (addr_dec (value_to_nat r) 2); simpl.
+    {
+    eapply hoare_triple_pimpl;
+    try solve [intros; simpl in *; eauto].
+    eapply hoare_triple_strengthen_pre;
+    [apply read_okay | intros; simpl; cancel].
+
+    {
+      intros; simpl.
+      eapply hoare_triple_weaken_post_weak.
+      eapply hoare_triple_weaken_crash_strong.
+      eapply hoare_triple_strengthen_pre.
+      apply ret_okay.
+      
+      intros; simpl in *.
+      destruct_lift H;
+        destruct_lift H0; cleanup;
+          cancel; eauto.
+      
+      intros; simpl in *.
+      destruct_lift H;
+        destruct_lift H0; cleanup;
+          cancel; eauto.
+
+      intros; simpl in *.
+      destruct_lift H;
+        destruct_lift H0;
+        destruct_lift H1;
+        cleanup;
+          cancel; eauto.
+    }
+    intros; simpl in *;
+      destruct_lift H;
+      destruct_lift H0; cleanup;
+        norm; [cancel| intuition (eauto; try omega)].
+    }
+
+    destruct (addr_dec (value_to_nat r) 3); simpl.
+    {
+    eapply hoare_triple_pimpl;
+    try solve [intros; simpl in *; eauto].
+    eapply hoare_triple_strengthen_pre;
+    [apply read_okay | intros; simpl; cancel].
+
+    {
+      intros; simpl.
+      eapply hoare_triple_weaken_post_weak.
+      eapply hoare_triple_weaken_crash_strong.
+      eapply hoare_triple_strengthen_pre.
+      apply ret_okay.
+      
+      intros; simpl in *.
+      destruct_lift H;
+        destruct_lift H0; cleanup;
+          cancel; eauto.
+      
+      intros; simpl in *.
+      destruct_lift H;
+        destruct_lift H0; cleanup;
+          cancel; eauto.
+
+      intros; simpl in *.
+      destruct_lift H;
+        destruct_lift H0;
+        destruct_lift H1;
+        cleanup;
+          cancel; eauto.
+    }
+    intros; simpl in *;
+      destruct_lift H;
+      destruct_lift H0; cleanup;
+        norm; [cancel| intuition (eauto; try omega)].
+    }
+
+      {
+      intros; simpl.
+      eapply hoare_triple_weaken_post_weak.
+      eapply hoare_triple_weaken_crash_strong.
+      eapply hoare_triple_strengthen_pre.
+      apply ret_okay.
+
+      eassign (F * rep dh * ⟦⟦ r = v ⟧⟧).
+      destruct_lift H;
+        cleanup.
+      intros; simpl in *; unfold rep; cancel.
+      
+      unfold rep; intros; simpl in *.
+      destruct_lift H;
+        cleanup.
+      norm; [cancel| intuition (eauto; try omega)].      
+
+      intros; simpl in *.
+      unfold rep;
+      destruct_lift H;
+        destruct_lift H0;
+        cleanup;
+      norm; [cancel| intuition (eauto; try omega)].
+      
+      left; split; eauto.
+      left.
+      destruct (addr_dec (value_to_nat v) 0).
+      destruct H8; eauto.
+      destruct (addr_dec (value_to_nat v) 1).
+      destruct H7; eauto.
+      omega.
+    }
+  }
+
+  {
+      intros; simpl.
+      eapply hoare_triple_weaken_post_weak.
+      eapply hoare_triple_weaken_crash_strong.
+      eapply hoare_triple_strengthen_pre.
+      apply ret_okay.
+      intros; simpl; rewrite emp_star_r; eauto.
+      destruct_lift H; cancel.
+      destruct_lift H; cancel.
+      left; intuition.      
+      right; omega.
+  }
+
+  intros; simpl.
+  destruct_lift H; cancel.
+Qed.
+
+Lemma exis_lift_absorb:
+  forall A AEQ V T (P: T -> @pred A AEQ V) Q,
+    (exists x, P x) * [[ Q ]] =p=> exists x, (P x * [[Q]]).
+Proof.
+  intros; cancel.
+Qed.
+*)
+
+Theorem write_ok:
+  forall dh a v,
+  << o >>
+   (rep dh)
+   (write a v)
+  << d, r >>
+   (exists dh',
+    rep dh' * [[ oracle_refines_to _ d (Write a v) o (Cont::nil) ]] *
+     [[(r = None /\ dh' = dh /\ dh a = None) \/
+       (r = Some tt /\ dh a <> None /\ dh' = upd dh a v)%type]])
+   (exists dh',
+    rep dh' *
+    [[((dh' = dh /\ oracle_refines_to _ d (Write a v) o (Crash1::nil)) \/
+       (dh a <> None /\ dh' = upd dh a v /\ oracle_refines_to _ d (Write a v) o (Crash2::nil)))%type]]).
+Proof. Admitted. (*
+  intros.
+  unfold write; simpl.
+
+  repeat (apply hoare_triple_pre_ex; intros).
+    eapply hoare_triple_pimpl;
+      try solve [intros; simpl in *; eauto].
+    eapply hoare_triple_strengthen_pre;
+      [apply read_okay | intros; simpl; cancel].
+    
+  intros; simpl; destruct (addr_dec a 1); subst.
+  {
+    intros; simpl.
+    destruct (addr_dec (value_to_nat r) 1); simpl.
+    {
+      eapply hoare_triple_pimpl;
+        try solve [intros; simpl in *; eauto].
+      eapply hoare_triple_strengthen_pre;
+        [apply write_okay | intros; simpl; cancel].
+      
+      {
+        intros; simpl.
+        eapply hoare_triple_weaken_post_weak.
+        eapply hoare_triple_weaken_crash_strong.
+        eapply hoare_triple_strengthen_pre.
+        apply ret_okay.
+        
+        intros; simpl in *.
+        rewrite <- emp_star_r; eauto.
+        
+        intros; unfold rep; simpl in *.
+        norm; [cancel|].
+        eassign (upd dh 1 v).
+        rewrite upd_eq'.
+        repeat rewrite upd_ne; eauto.
+        destruct_lift H;
+          destruct_lift H0;
+          cleanup;
+          intuition (eauto; try omega).
+        rewrite upd_ne; eauto; omega.
+        right; intuition eauto.
+        cleanup.
+
+        intros; unfold rep; simpl in *.
+        norm; [cancel|].
+        eassign (upd dh 1 v).
+        rewrite upd_eq'.
+        repeat rewrite upd_ne; eauto.
+        destruct_lift H;
+          destruct_lift H0;
+          cleanup;
+          intuition (eauto; try omega).
+        rewrite upd_ne; eauto; omega.
+        right; intuition eauto.
+        cleanup.
+      }        
+      intros; unfold rep; simpl in *.
+      destruct_lift H;
+          destruct_lift H0;
+          cleanup;
+        norm; [cancel| intuition (eauto; try omega)].
+    }
+
+    destruct (addr_dec (value_to_nat r) 3); simpl.
+    {
+      eapply hoare_triple_pimpl;
+        try solve [intros; simpl in *; eauto].
+      eapply hoare_triple_strengthen_pre;
+        [apply write_okay | intros; simpl; cancel].
+      {
+        intros; simpl.
+        eapply hoare_triple_weaken_post_weak.
+        eapply hoare_triple_weaken_crash_strong.
+        eapply hoare_triple_strengthen_pre.
+        apply ret_okay.
+        
+        intros; simpl in *.
+        rewrite <- emp_star_r; eauto.
+        
+        intros; unfold rep; simpl in *.
+        norm; [cancel|].
+        eassign (upd dh 1 v).
+        rewrite upd_eq'.
+        repeat rewrite upd_ne; eauto.
+        destruct_lift H;
+          destruct_lift H0;
+          cleanup;
+          intuition (eauto; try omega).
+        rewrite upd_ne; eauto; omega.
+        right; intuition eauto.
+        cleanup.
+
+        intros; unfold rep; simpl in *.
+        norm; [cancel|].
+        eassign (upd dh 1 v).
+        rewrite upd_eq'.
+        repeat rewrite upd_ne; eauto.
+        destruct_lift H;
+          destruct_lift H0;
+          cleanup;
+          intuition (eauto; try omega).
+        rewrite upd_ne; eauto; omega.
+        right; intuition eauto.
+        cleanup.
+      }        
+      intros; unfold rep; simpl in *.
+      destruct_lift H;
+          destruct_lift H0;
+          cleanup;
+        norm; [cancel| intuition (eauto; try omega)].
+    }
+
+      {
+      intros; simpl.
+      eapply hoare_triple_weaken_post_weak.
+      eapply hoare_triple_weaken_crash_strong.
+      eapply hoare_triple_strengthen_pre.
+      apply ret_okay.
+
+      eassign (F * rep dh).
+      destruct_lift H;
+        cleanup.
+      intros; simpl in *; unfold rep; cancel.
+
+      cancel.
+      cancel.
+    }
+  }
+  
+
+  destruct (addr_dec a 2); subst.
+   {
+    intros; simpl.
+    destruct (addr_dec (value_to_nat r) 2); simpl.
+    {
+      eapply hoare_triple_pimpl;
+        try solve [intros; simpl in *; eauto].
+      eapply hoare_triple_strengthen_pre;
+        [apply write_okay | intros; simpl; cancel].
+      destruct_lift H; cleanup.
+      
+      {
+        intros; simpl.
+        eapply hoare_triple_weaken_post_weak.
+        eapply hoare_triple_weaken_crash_strong.
+        eapply hoare_triple_strengthen_pre.
+        apply ret_okay.
+
+        intros; simpl in *.
+        rewrite <- emp_star_r; eauto.
+        
+        intros; unfold rep; simpl in *.
+        norm; [cancel|].
+        eassign (upd dh 2 v).
+        rewrite upd_eq'.
+        repeat rewrite upd_ne; eauto.
+        destruct_lift H;
+          destruct_lift H0;
+          cleanup;
+          intuition (eauto; try omega).
+        rewrite upd_ne; eauto; omega.
+        right; intuition eauto.
+        cleanup.
+
+        intros; unfold rep; simpl in *.
+        norm; [cancel|].
+        eassign (upd dh 2 v).
+        rewrite upd_eq'.
+        repeat rewrite upd_ne; eauto.
+        destruct_lift H;
+          destruct_lift H0;
+          cleanup;
+          intuition (eauto; try omega).
+        rewrite upd_ne; eauto; omega.
+        right; intuition eauto.
+        cleanup.
+      }        
+      intros; unfold rep; simpl in *.
+      destruct_lift H;
+          destruct_lift H0;
+          cleanup;
+        norm; [cancel| intuition (eauto; try omega)].
+    }
+
+    destruct (addr_dec (value_to_nat r) 3); simpl.
+    {
+      eapply hoare_triple_pimpl;
+        try solve [intros; simpl in *; eauto].
+      eapply hoare_triple_strengthen_pre;
+        [apply write_okay | intros; simpl; cancel].
+      {
+        intros; simpl.
+        eapply hoare_triple_weaken_post_weak.
+        eapply hoare_triple_weaken_crash_strong.
+        eapply hoare_triple_strengthen_pre.
+        apply ret_okay.
+        
+        intros; simpl in *.
+        rewrite <- emp_star_r; eauto.
+        
+        intros; unfold rep; simpl in *.
+        norm; [cancel|].
+        eassign (upd dh 2 v).
+        rewrite upd_eq'.
+        repeat rewrite upd_ne; eauto.
+        destruct_lift H;
+          destruct_lift H0;
+          cleanup;
+          intuition (eauto; try omega).
+        rewrite upd_ne; eauto; omega.
+        right; intuition eauto.
+        cleanup.
+
+        intros; unfold rep; simpl in *.
+        norm; [cancel|].
+        eassign (upd dh 2 v).
+        rewrite upd_eq'.
+        repeat rewrite upd_ne; eauto.
+        destruct_lift H;
+          destruct_lift H0;
+          cleanup;
+          intuition (eauto; try omega).
+        rewrite upd_ne; eauto; omega.
+        right; intuition eauto.
+        cleanup.
+      }        
+      intros; unfold rep; simpl in *.
+      destruct_lift H;
+          destruct_lift H0;
+          cleanup;
+        norm; [cancel| intuition (eauto; try omega)].
+    }
+
+      {
+      intros; simpl.
+      eapply hoare_triple_weaken_post_weak.
+      eapply hoare_triple_weaken_crash_strong.
+      eapply hoare_triple_strengthen_pre.
+      apply ret_okay.
+
+      eassign (F * rep dh).
+      destruct_lift H;
+        cleanup.
+      intros; simpl in *; unfold rep; cancel.
+
+      cancel.
+      cancel.
+
+      }
+   }
+
+   {
+      intros; simpl.
+      eapply hoare_triple_weaken_post_weak.
+      eapply hoare_triple_weaken_crash_strong.
+      eapply hoare_triple_strengthen_pre.
+      apply ret_okay.
+
+      eassign (F * rep dh).
+      destruct_lift H;
+        cleanup.
+      intros; simpl in *; unfold rep; cancel.
+      
+      all: cancel.
+   }
+   intros; simpl in *;
+     destruct_lift H; cleanup.
+   cancel; unfold rep; cancel.
+Qed.
+*)
+
+
+
+Theorem free_ok:
+  forall dh a,
+  << o >>
+   (rep dh)
+   (free a)
+  << d, r >>
+   (rep (delete dh a) *
+    [[ oracle_refines_to _ d (Free a) o (Cont::nil) ]])
+   (exists dh',
+       rep dh' *
+       [[ (dh' = dh /\ oracle_refines_to _ d (Free a) o (Crash1::nil)) \/
+          (dh' = (delete dh a) /\ oracle_refines_to _ d (Free a) o (Crash2::nil))]]).
+Proof. Admitted. (*
+  intros.
+  unfold free; simpl.
+
+  destruct (addr_dec a 1); subst.
+  {
+    
+
+    intros; simpl.
+    eapply hoare_triple_pimpl;
+      try solve [intros; simpl in *; eauto].
+    eapply hoare_triple_strengthen_pre;
+      [apply unseal_okay | intros; simpl; cancel].
+    apply upd_eq; eauto.
+    simpl; apply can_access_public.
+
+    intros; simpl.
+    destruct (addr_dec (value_to_nat r0) 1); simpl.
+    {
+      eapply hoare_triple_pimpl;
+        try solve [intros; simpl in *; eauto].
+      eapply hoare_triple_strengthen_pre;
+        [apply seal_okay | intros; simpl; cancel].
+    
+      {
+        intros; simpl.
+        eapply hoare_triple_weaken_post_weak.
+        eapply hoare_triple_weaken_crash_strong.
+        eapply hoare_triple_strengthen_pre.
+        apply write_okay.
+        
+        intros; simpl in *.
+        cancel.
+        apply upd_eq'.
+        
+        intros; simpl in *.
+        norm; [cancel|].
+        eassign dh.
+        destruct_lift H;
+          destruct_lift H0;
+          destruct_lift H1;
+          cleanup;
+          intuition (eauto; try omega).
+
+        intros; simpl in *.
+        norm; [cancel|].
+        rewrite delete_eq.
+        repeat rewrite delete_ne; eauto.
+        rewrite nat_to_value_to_nat.
+        destruct_lift H;
+          destruct_lift H0;
+          destruct_lift H1;
+          cleanup;
+          intuition (eauto; try omega).
+        rewrite delete_ne; eauto; omega.
+      }        
+      intros; simpl in *.
+      destruct_lift H;
+          destruct_lift H0;
+          destruct_lift H1;
+          cleanup;
+        norm; [cancel| intuition (eauto; try omega)].
+    }
+
+    destruct (addr_dec (value_to_nat r0) 3); simpl.
+    {
+      eapply hoare_triple_pimpl;
+        try solve [intros; simpl in *; eauto].
+      eapply hoare_triple_strengthen_pre;
+        [apply seal_okay | intros; simpl; cancel].
+    
+      {
+        intros; simpl.
+        eapply hoare_triple_weaken_post_weak.
+        eapply hoare_triple_weaken_crash_strong.
+        eapply hoare_triple_strengthen_pre.
+        apply write_okay.
+        
+        intros; simpl in *.
+        cancel.
+        apply upd_eq'.
+        
+        intros; simpl in *.
+        norm; [cancel|].
+        eassign dh.
+        destruct_lift H;
+          destruct_lift H0;
+          destruct_lift H1;
+          cleanup;
+          intuition (eauto; try omega).
+
+        intros; simpl in *.
+        norm; [cancel|].
+        rewrite delete_eq.
+        repeat rewrite delete_ne; eauto.
+        rewrite nat_to_value_to_nat.
+        destruct_lift H;
+          destruct_lift H0;
+          destruct_lift H1;
+          cleanup;
+          intuition (eauto; try omega).
+        rewrite delete_ne; eauto; omega.
+      }        
+      intros; simpl in *.
+      destruct_lift H;
+          destruct_lift H0;
+          destruct_lift H1;
+          cleanup;
+        norm; [cancel| intuition (eauto; try omega)].
+    }
+
+    {
+      {
+        intros; simpl.
+        eapply hoare_triple_weaken_post_weak.
+        eapply hoare_triple_weaken_crash_strong.
+        eapply hoare_triple_strengthen_pre.
+        apply ret_okay.
+        
+        intros; simpl in *.
+        eassign (((((0 |-> (Public, v, v0) ✶ F) ✶ 1 |-> v1) ✶ 2 |-> v2) ✶ (⟦⟦ r0 = v ⟧⟧))).
+        cancel.
+        
+        intros; simpl in *.
+        norm; [cancel|].
+        eassign dh.
+        destruct_lift H;
+          destruct_lift H0;
+          cleanup;
+          intuition (eauto; try omega).
+
+        intros; simpl in *.
+        norm; [cancel|].
+        rewrite delete_eq.
+        repeat rewrite delete_ne; eauto.
+        destruct_lift H;
+          destruct_lift H0;
+          destruct_lift H1;
+          cleanup;
+          intuition (eauto; try omega).
+        rewrite delete_ne; eauto; omega.
+      }
+    }
+    
+      intros; simpl in *;
+      destruct_lift H;
+          destruct_lift H0;
+          cleanup;
+          norm; [cancel| intuition (eauto; try omega)].
+    intros; simpl in *;
+      destruct_lift H;
+          cleanup;
+        norm; [cancel| intuition (eauto; try omega)].
+  }
+
+  destruct (addr_dec a 2); subst.
+  {
+    unfold rep.
+    repeat (apply hoare_triple_pre_ex; intros).
+    eapply hoare_triple_pimpl;
+      try solve [intros; simpl in *; eauto].
+    eapply hoare_triple_strengthen_pre;
+      [apply read_okay | intros; simpl; cancel].
+
+    intros; simpl.
+    eapply hoare_triple_pimpl;
+      try solve [intros; simpl in *; eauto].
+    eapply hoare_triple_strengthen_pre;
+      [apply unseal_okay | intros; simpl; cancel].
+    apply upd_eq; eauto.
+    simpl; apply can_access_public.
+
+    intros; simpl.
+    destruct (addr_dec (value_to_nat r0) 2); simpl.
+    {
+      eapply hoare_triple_pimpl;
+        try solve [intros; simpl in *; eauto].
+      eapply hoare_triple_strengthen_pre;
+        [apply seal_okay | intros; simpl; cancel].
+    
+      {
+        intros; simpl.
+        eapply hoare_triple_weaken_post_weak.
+        eapply hoare_triple_weaken_crash_strong.
+        eapply hoare_triple_strengthen_pre.
+        apply write_okay.
+        
+        intros; simpl in *.
+        cancel.
+        apply upd_eq'.
+        
+        intros; simpl in *.
+        norm; [cancel|].
+        eassign dh.
+        destruct_lift H;
+          destruct_lift H0;
+          destruct_lift H1;
+          cleanup;
+          intuition (eauto; try omega).
+
+        intros; simpl in *.
+        norm; [cancel|].
+        rewrite delete_eq.
+        repeat rewrite delete_ne; eauto.
+        rewrite nat_to_value_to_nat.
+        destruct_lift H;
+          destruct_lift H0;
+          destruct_lift H1;
+          cleanup;
+          intuition (eauto; try omega).
+        rewrite delete_ne; eauto; omega.
+      }        
+      intros; simpl in *.
+      destruct_lift H;
+          destruct_lift H0;
+          destruct_lift H1;
+          cleanup;
+        norm; [cancel| intuition (eauto; try omega)].
+    }
+
+    destruct (addr_dec (value_to_nat r0) 3); simpl.
+    {
+      eapply hoare_triple_pimpl;
+        try solve [intros; simpl in *; eauto].
+      eapply hoare_triple_strengthen_pre;
+        [apply seal_okay | intros; simpl; cancel].
+    
+      {
+        intros; simpl.
+        eapply hoare_triple_weaken_post_weak.
+        eapply hoare_triple_weaken_crash_strong.
+        eapply hoare_triple_strengthen_pre.
+        apply write_okay.
+        
+        intros; simpl in *.
+        cancel.
+        apply upd_eq'.
+        
+        intros; simpl in *.
+        norm; [cancel|].
+        eassign dh.
+        destruct_lift H;
+          destruct_lift H0;
+          destruct_lift H1;
+          cleanup;
+          intuition (eauto; try omega).
+
+        intros; simpl in *.
+        norm; [cancel|].
+        rewrite delete_eq.
+        repeat rewrite delete_ne; eauto.
+        rewrite nat_to_value_to_nat.
+        destruct_lift H;
+          destruct_lift H0;
+          destruct_lift H1;
+          cleanup;
+          intuition (eauto; try omega).
+        rewrite delete_ne; eauto; omega.
+      }        
+      intros; simpl in *.
+      destruct_lift H;
+          destruct_lift H0;
+          destruct_lift H1;
+          cleanup;
+        norm; [cancel| intuition (eauto; try omega)].
+    }
+
+    {
+      {
+        intros; simpl.
+        eapply hoare_triple_weaken_post_weak.
+        eapply hoare_triple_weaken_crash_strong.
+        eapply hoare_triple_strengthen_pre.
+        apply ret_okay.
+        
+        intros; simpl in *.
+        eassign (((((0 |-> (Public, v, v0) ✶ F) ✶ 1 |-> v1) ✶ 2 |-> v2) ✶ (⟦⟦ r0 = v ⟧⟧))).
+        cancel.
+        
+        intros; simpl in *.
+        norm; [cancel|].
+        eassign dh.
+        destruct_lift H;
+          destruct_lift H0;
+          cleanup;
+          intuition (eauto; try omega).
+
+        intros; simpl in *.
+        norm; [cancel|].
+        rewrite delete_eq.
+        repeat rewrite delete_ne; eauto.
+        destruct_lift H;
+          destruct_lift H0;
+          destruct_lift H1;
+          cleanup;
+          intuition (eauto; try omega).
+        rewrite delete_ne; eauto; omega.
+      }
+    }
+    
+      intros; simpl in *;
+      destruct_lift H;
+          destruct_lift H0;
+          cleanup;
+          norm; [cancel| intuition (eauto; try omega)].
+    intros; simpl in *;
+      destruct_lift H;
+          cleanup;
+        norm; [cancel| intuition (eauto; try omega)].
+  }
+
+
+  {
+    intros; simpl.
+    eapply hoare_triple_weaken_post_weak.
+    eapply hoare_triple_weaken_crash_strong.
+    eapply hoare_triple_strengthen_pre.
+    apply ret_okay.
+
+    all: cancel.
+    cancel.
+    unfold rep.
+    destruct a.
+    unfold delete at 1.
+    destruct (addr_dec 0 0); intuition.
+    repeat rewrite delete_ne; eauto.
+    cancel.
+    rewrite delete_ne; eauto.
+    omega.
+
+    repeat rewrite delete_ne; eauto.
+    cancel.
+    destruct (addr_dec (S a) n1); subst.
+    apply delete_eq.
+    rewrite delete_ne; eauto.
+  }
+Qed.
+*)
