src/Layer1to2RefinementDefinitions.v
@@ -1,0 +1,96 @@
+Require Import Primitives Layer1 Layer2 BlockAllocatorDefinitions.
+Close Scope pred_scope.
+Import ListNotations.
+
+Fixpoint compile {T} (p2: Layer2.prog T) : Layer1.prog T :=
+    match p2 with
+    | Read a => read a
+    | Write a v => write a v
+    | Alloc v => alloc v
+    | Free a => free a
+    | Ret v => Layer1.Ret v
+    | Bind px py => Layer1.Bind (compile px) (fun x => compile (py x))
+    end.
+
+(* October 12: I need oracle_ok in here because specifications of block allocator requires it as a precondition *)
+  Fixpoint oracle_refines_to T (d1: Layer1.state) (p: Layer2.prog T)  (o1: Layer1.oracle) (o2: Layer2.oracle) : Prop :=
+    oracle_ok (compile p) o1 d1 /\
+    match p with
+    | Alloc v =>
+      if (in_dec Layer1.token_dec Layer1.Crash o1) then
+        forall d1',
+          Layer1.exec o1 d1 (compile p) (Crashed d1') ->
+          let sv := Disk.read d1 0 in
+          let sv' := Disk.read d1' 0 in
+          match sv, sv' with
+          | Some v, Some v' =>
+            (v = v' ->
+             o2 = [Crash1]) /\
+            (v <> v' ->
+             let bits := bits (value_to_bits v) in
+             let index := get_first_zero bits in
+             o2 = [CrashAlloc index])
+          | _, _ => False
+          end
+      else
+        let sv := Disk.read d1 0 in
+        match sv with
+        | Some v =>
+          let bits := bits (value_to_bits v) in
+          let index := get_first_zero bits in
+          
+          if Compare_dec.lt_dec index block_size then
+            o2 = [BlockNum index]
+          else
+            o2 = [DiskFull]
+        | None => False
+        end
+    | @Bind T1 T2 p1 p2 =>
+      exists o1' o1'',
+      o1 = o1'++o1'' /\
+      (forall d1', Layer1.exec o1 d1 (compile p1) (Crashed d1') ->
+         oracle_refines_to T1 d1 p1 o1 o2 /\ o1'' = []) /\
+      (forall d1' r,
+         Layer1.exec o1' d1 (compile p1) (Finished d1' r) ->
+         exists o2' o2'',
+         oracle_refines_to T1 d1 p1 o1' o2' /\
+         oracle_refines_to T2 d1' (p2 r) o1'' o2'' /\
+         o2 = o2' ++ o2'')
+    | Read _ =>
+      if (in_dec Layer1.token_dec Layer1.Crash o1) then
+        o2 = [Crash1]
+      else
+        o2 = [Cont]
+    | Ret _ =>
+      if (in_dec Layer1.token_dec Layer1.Crash o1) then
+        o2 = [Crash1]
+      else
+        o2 = [Cont]
+    | Free _ =>
+      if (in_dec Layer1.token_dec Layer1.Crash o1) then
+        o2 = [Crash1]
+      else
+        o2 = [Cont]
+    | Write a _ =>
+      if (in_dec Layer1.token_dec Layer1.Crash o1) then
+         forall d1',
+          Layer1.exec o1 d1 (compile p) (Crashed d1') ->
+          let sv := d1 a in
+          let sv' := d1' a in
+          match sv, sv' with
+          | Some v, Some v' =>
+            (v = v' ->
+             o2 = [Crash1]) /\
+            (v <> v' ->
+             o2 = [Crash2])
+          | _, _ => False
+          end
+      else
+        o2 = [Cont]
+    end.
+
+  Definition refines_to d1 d2 :=
+    exists F, (F * rep d2)%pred d1.
+
+  Definition compilation_of T p1 p2 :=
+    p1 = @compile T p2.
