Problems.md
@@ -1,0 +1,16 @@
+#### Problems
+
+1. Because low's crash point is nondeterministic, high's crash result becomes nondeterministic.
+
+   When proving BS in high -> low direction, we can't make sure low exec also crashes at the same point.
+
+   - Solution: Add what oracle refines to to specs of low so you will know exactly the high oracle for that execution.
+
+   
+
+2. When high state changes during an exec, we can't prove new one is valid.
+
+   - Solution: Remove validity relations from definitions.
+     - Conclusion: Won't work because I need it for data noninterference. If I don't say state is valid but try to prove from an arbitrary state, it won't work.
+   - ???
+
